Using \eqref{general_model},  
\beno
-\mbE \, \nabla_{\nat}^2 \, \ell(\nat; \bX, \bY)
\= \dsum_{\by \in \mbY} \, \dsum_{\bx \in \mbX} \, - \nabla_{\nat}^2 \, \ell(\nat; \bx, \by) \, 
\sepmodel(\bX = \bx \,|\, \bY = \by) \, g(\by) \s \\ 
\= \dsum_{\by \in \mbY} \, g(\by)  \dsum_{\bx \in \mbX} \, - \nabla_{\nat}^2 \, \ell(\nat; \bx, \by) \, 
\sepmodel(\bX = \bx \,|\, \bY = \by) \s \\ 
\= \dsum_{\by \in \mbY} \, g(\by) \, \dsum_{\{i,j\} \subset \mN \,:\, y_{i,j} = 1} \, \mcI(\nat) \s \\ 
\= \mcI(\nat) \, \dsum_{\by \in \mbY} \, g(\by)  \, \norm{\by}_1 \s\\
\= \mcI(\nat) \, \mbE \norm{\bY}_1.  
\ee
The above follows by 
exploiting the conditional independence of vectors $\bx_{i,j}$ ($\{i,j\} \subset \mN$) 
given $\bY = \by$ under \eqref{general_model}, 
which implies 
\beno
\ell(\nat; \bx, \by)
\= \dsum_{\{i,j\} \subset \mN} \log \sepmodel(\bX_{i,j} = \bx_{i,j} \,|\, \bY = \by), 
\ee
and from the fact that the conditional probability distribution of $\bX_{i,j}$ 
given $\bY$ 
is a degenerate point mass at $\bm{0}$ 
when $Y_{i,j} = 0$ so that $- \nabla_{\nat}^2 \, \ell(\nat; \bx, \by)$ is a sum of $\norm{\by}_1$ 
matrices each equal to $\mcI(\nat)$,
i.e.,
given $\by \in \mbY$,
we have 
\beno
&& \dsum_{\bx \in \mbX} - \nabla_{\nat}^2 \, \ell(\nat; \bx, \by) \, \sepmodel(\bX = \bx \,|\, \bY = \by) \s\\ 
\= \dsum_{\{i,j\} \subset \mN} \, \mbE\left[- \nabla_{\nat}^2 \, L_{i,j}(\nat, \bX_{i,j}, \bY) \,|\, \bY = \by \right]  
\;\;= \dsum_{\{i,j\} \subset \mN \,:\, y_{i,j} = 1} \, \mcI(\nat). 
\ee
The fact that $\mcI(\nat)$ is constant for all pairs $\{i,j\} \subset \mN$ satisfying $Y_{i,j} = 1$ 
follows from the form of \eqref{general_model},
which assumes each vector $\bX_{i,j}$ ($\{i,j\} \subset \mN$)
is conditionally independent and identically distributed, 
conditional on $\bY$.  
Hence, 
\beno
\mbE \left[ -\nabla_{\nat}^2 \, \ell(\nat; \bX, \bY)  \right]
\= \mcI(\nat) \, \mbE \, \norm{\bY}_1,
\ee 
which in turn implies 
\beno
\lambda_{\min}(-\mbE \nabla_{\nat}^2 \,\ell(\nat; \bX, \bY)) = \lambda_{\min}(\mcI(\nat)) \, \mbE \, \norm{\bY}_1\s\\
\lambda_{\max}(-\mbE \nabla_{\nat}^2 \,\ell(\nat; \bX, \bY)) = \lambda_{\max}(\mcI(\nat)) \, \mbE \, \norm{\bY}_1.
\ee

\qed 
