Our proof follows a similar scheme as in the proof of \Cref{lem:leader-bellman-loss}.

\paragraph{Concentration.}
We first take
\begin{align*}
    {Z_h^i} &= \ell_{h}(U'_{h}, U_{h + 1}, \theta_{h+1}, \pi) - \ell_{h}(\TT_{h}^{*,\theta}U_{h + 1}, U_{h + 1}, \theta_{h+1}, \pi)\nend
    & = \rbr{U_h(s_h^i, a_h^i, b_h^i) - u_h^i -  T_{h+1}^{*, \theta} U_{h+1}(s_{h+1}^i)}^2  - \rbr{\TT_h^{*, \theta} U_{h+1}(s_h^i, a_h^i, b_h^i) - u_h^i - T_{h+1}^{*, \theta} U_{h+1}(s_{h+1}^i)}^2.
\end{align*}
For the online setting, we have $(s_h^i, a_h^i, b_h^i, s_{h+1}^i)$ adapted to some filtration $\cF_h^i$. One choice of the filtration is $\cF_h^j=\sigma\rbr{\tau^{1:j-1}}$. Another choice of the filtration is $\cF_h^j=\sigma\rbr{(s_h^j, a_h^j, b_h^j), (s_h^i, a_h^i, b_h^i, s_{h+1}^i)_{i\in[j-1]}}$, where $\sigma(X)$ is the sigma-algebra of $X$.
They will both work for our proof.
We let $\EE^{i}_{x}[\cdot]$ be a short hand of $\EE^{i}[\cdot\given x, \cF_h^i]$ in the following proof.
We first calculate the expectation, 
\begin{align*}
    \EE^{i}[{Z_h^i}] 
    &= \EE^{i} \bigg[\EE^{i}_{s_h^i, a_h^i, b_h^i} \Big[\rbr{U_h(s_h^i, a_h^i, b_h^i) - u_h^i -  T_{h+1}^{*, \theta} U_{h+1}(s_{h+1}^i)}^2  \nend
    &\qquad - \rbr{\TT_h^{*, \theta} U_{h+1}(s_h^i, a_h^i, b_h^i) - u_h^i - T_{h+1}^{*, \theta} U_{h+1}(s_{h+1}^i)}^2\Big]\bigg]\nend
    & = \EE^{i}\bigg[\Bigrbr{U_h(s_h^i, a_h^i, b_h^i)- \TT_h^{*, \theta} U_{h+1}(s_h^i, a_h^i, b_h^i)}\nend
    &\qquad \cdot \EE^{i}_{s_h^i, a_h^i, b_h^i}\sbr{U_h(s_h^i, a_h^i, b_h^i) + \TT_h^{*, \theta} U_{h+1}(s_h^i, a_h^i, b_h^i)- 2u_h^i - 2T_{h+1}^{*, \theta} U_{h+1}(s_{h+1}^i) }\bigg]\nend
    & = \EE^{i}\sbr{\Bigrbr{U_h(s_h^i, a_h^i, b_h^i)- \TT_h^{*, \theta} U_{h+1}(s_h^i, a_h^i, b_h^i)}^2}, 
\end{align*}
where the second equality holds by the law of total expectation, and the third equality holds by noting that $\EE^{i}_{s_h^i, a_h^i, b_h^i}\osbr{u_h^i  + T_{h+1}^{*, \theta} U_{h+1}(s_{h+1}^i)} = \TT_h^{*, \theta} U_{h+1} (s_h^i, a_h^i, b_h^i)$.
Next, we calculate the variance, 
\begin{align*}
    \Var^{i}[{Z_h^i}^2] &\le \EE^{i}[{Z_h^i}^2]\nend
    &\le \EE^{i}\bigg[\Bigrbr{U_h(s_h^i, a_h^i, b_h^i)- \TT_h^{*, \theta} U_{h+1}(s_h^i, a_h^i, b_h^i)}^2\nend
    &\qquad \cdot \EE^{i}_{s_h^i, a_h^i, b_h^i}\sbr{\rbr{U_h(s_h^i, a_h^i, b_h^i) + \TT_h^{*, \theta} U_{h+1}(s_h^i, a_h^i, b_h^i)- 2u_h^i - 2T_{h+1}^{*, \theta} U_{h+1}(s_{h+1}^i)}^2 } \bigg]\nend
    &\le 49 B_U^2 \EE^{i}\sbr{\Bigrbr{U_h(s_h^i, a_h^i, b_h^i)- \TT_h^{*, \theta} U_{h+1}(s_h^i, a_h^i, b_h^i)}^2} = 49 B_U^2 \EE^{i}[{Z_h^i}].
\end{align*}
Also, one can verify that $|{Z_h^i}|\le 9B_U^2$ where $B_U$ bounds both the leader's reward and the value function class $\cU$.
We next take a $\epsilon$-covering of the class $\cZ_h=\cU^2\times\Theta_{h+1}$ with respect to the following distance defined in \eqref{eq:rho-cZ},
\begin{align*}
    &\rho\orbr{z, \tilde z}  = \max_{h\in[H]}\cbr{\bignbr{U_h-\tilde U_h}_\infty, \bignbr{ T_{h+1}^{*,\theta} U_{h+1} (\cdot) -  T_{h+1}^{*,\tilde\theta} \tilde U_{h+1} (\cdot)}_\infty }, 
\end{align*} 
We invoke the Freedman inequality \Cref{lem:freedman} for the martingale sequence $Z_h^i -\EE^i[Z_h^i]$, which says that for all $t\in [T], h\in[H], z\in\cZ_\epsilon$, it holds with probability at least $1-\delta$
\begin{align*}
    \sum_{i=1}^t \rbr{Z_h^i - \EE^i[Z_h^i]}
    &\le \frac{\lambda(e-2)}{9 B_U^2} \sum_{i=1}^t \EE^i\sbr{\rbr{Z_h^i - \EE^i[Z_h^i]}^2} + 9 \lambda^{-1} B_U^2\log(TH\cN_\rho(\cZ_h, \epsilon)\delta^{-1})\nend
    &\le \frac{\lambda(e-2) 49 }{9 } \sum_{i=1}^t \EE^i\sbr{Z_h^i} + 9 \lambda^{-1} B_U^2\log(TH\cN_\rho(\cZ_h, \epsilon)\delta^{-1}), \quad \forall \lambda\in(0, 1).
\end{align*}
Here, we plug in $\lambda = 9/98(e-2)$, $\epsilon=T^{-1}$ and notice that the above inequality also holds for $-Z_h^i + \EE^i[Z_h^i]$, which gives us for all $z\in\cZ_\epsilon, h\in[H], t\in[T]$ that
\begin{align}\label{eq:leader-Bellman-1}
    \abr{\sum_{i=1}^t \rbr{Z_h^i - \EE^i[Z_h^i]}} \le \frac 1 2 \sum_{i=1}^t \EE^i\sbr{Z_h^i} + c B_U^2\log(TH\cN_\rho(\cZ_h, T^{-1})\delta^{-1}), 
\end{align}
where we plug in $\epsilon=T^{-1}$ and $c=98(e-2)$ should be a universal constant. 
Next, we notice that
\begin{align*}
    &\bigrbr{U_h(s_h^i, a_h^i, b_h^i) - u_h^i -  T_{h+1}^{*,\theta} U_{h+1}(s_{h+1}^i)}^2  - \bigrbr{\TT_h^{*, \theta} U_{h+1}(s_h^i, a_h^i, b_h^i) - u_h^i - T_{h+1}^{*,\theta} U_{h+1}(s_{h+1}^i)}^2 \nend
    &\qquad - \rbr{\bigrbr{\tilde U_h(s_h^i, a_h^i, b_h^i) - u_h^i -  T_{h+1}^{*,\tilde\theta} \tilde U_{h+1}(s_{h+1}^i)}^2  - \bigrbr{\TT_h^{*, \tilde\theta} \tilde U_{h+1}(s_h^i, a_h^i, b_h^i) - u_h^i - T_{h+1}^{*,\tilde\theta} \tilde U_{h+1}(s_{h+1}^i)}^2}\nend
    %%%%%%%%%%%%%
    &\quad \le 6 B_U \rbr{\onbr{U-\tilde U}_\infty + \bignbr{(T_{h+1}^{*,\theta}-T_{h+1}^{*,\tilde\theta} )\tilde U_{h+1}}_\infty + \bignbr{T_{h+1}^{*,\theta}(U_{h+1} - \tilde U_{h+1})}_\infty}\nend
    &\qquad + 6 B_U \cdot 2\rbr{\bignbr{(T_{h+1}^{*,\theta}-T_{h+1}^{*,\tilde\theta} )\tilde U_{h+1}}_\infty + \bignbr{T_{h+1}^{*,\theta}(U_{h+1} - \tilde U_{h+1})}}\nend
    &\quad\le 6 B_U(2\epsilon + B_U \epsilon ) + 12 B_U(B_U\epsilon + \epsilon) \le (18 B_U^2 + 24 B_U)\epsilon, 
\end{align*}
Now, we let $\epsilon_S=c B_U^2 \allowbreak \log(TH\cN_\rho(\cZ_h, T^{-1})\delta^{-1}) + (45 B_U^2 + 60 B_u)$ and extend the result in \eqref{eq:leader-Bellman-1} to the whole class $\cY$, 
\begin{align*}
    \abr{\sum_{i=1}^t \rbr{Z_h^i - \EE^i[Z_h^i]}} 
    &\le \frac 1 2 \sum_{i=1}^t \EE^i\sbr{Z_h^i} + c B_U^2\log(TH\cN_\rho(\cZ, T^{-1})\delta^{-1}) + 2.5\cdot(18 B_U^2 + 24 B_U)\nend
    &\le \frac 1 2 \sum_{i=1}^t \EE^i\sbr{Z_h^i} + \epsilon_S.
\end{align*}
the following argument follows exactly the same as \eqref{eq:Bellman-loss-guarantee-1} and \eqref{eq:Bellman-loss-guarantee-2}, 
where we use the realizability assumption that $U^{*,\theta}\in \cU$ and the completeness assumption that there exists $U'\in\cU$ such that $U'=\TT_h^{*, \theta} U$ for any $U\in\cU, \theta\in\Theta$. 
We finish our proof of \Cref{lem:CI-U-online}.