





\iffalse
\subsection{Limiting flow}

Rewrite 
\[\beta_k (\vm_k - \vm_{k-1})= (1-\beta_k) (\vg_{k-1}-\vm_k)\]

So
\begin{align}
    \vx_k & = \vx_0 - \sum_{s=1}^k \eta_s \vm_s\\
    &= \vx_0 - \sum_{s=1}^k \eta_s \vg_{s-1} + \sum_{s=1}^k \eta_s\frac{\beta_s}{1-\beta_s}(\vm_s-\vm_{s-1})\\
\end{align}

Expanding $\Phi(\vx_k)$ gives  (for some $\vx'_{k-1},\vx''_{k-1}\in I[\vx_k,\vx_{k-1}]$)

\begin{align}
    \Phi(\vx_k) - \Phi(\vx_{k-1}) & = -\eta_k\dotp{\nabla\Phi(\vx_{k-1})}{\vm_k} + \frac{1}{2}\eta^2_k\nabla^2\Phi(\vx'_{k-1})[\vm_k,\vm_k]\\
    & = -\eta_k\dotp{\nabla\Phi(\vx_{k-1})}{\vg_{k-1}} +\frac{\eta_k\beta_k}{1-\beta_k}\dotp{\nabla\Phi(\vx_{k-1})}{\vm_{k}-\vm_{k-1}}+ \frac{1}{2}\eta^2_k\nabla^2\Phi(\vx'_{k-1})[\vm_k,\vm_k]\\
    & = -\eta_k\dotp{\nabla\Phi(\vx_{k-1})}{\vsigma_{\vxi_{k-1}}(\vx_{k-1})} +\frac{\eta_k\beta_k}{1-\beta_k}\dotp{\nabla\Phi(\vx_{k-1})}{\vm_{k}-\vm_{k-1}}+ \frac{1}{2}\eta^2_k\nabla^2\Phi(\vx'_{k-1})[\vm_k,\vm_k]\\
\end{align}

Therefore let $\mu_k =\frac{\eta_k\beta_k}{1-\beta_k}$
\begin{align}
    \Phi(\vx_k) & =\Phi(\vx_0)  -\sum_{s=1}^k \eta_s\dotp{\nabla\Phi_{s-1}}{\vsigma_{s-1}} +\sum_{s=1}^k\mu_s\dotp{\nabla\Phi_{s-1}}{\vm_{s}-\vm_{s-1}}+ \sum_{s=1}^k\frac{1}{2}\eta^2_s\nabla^2\Phi(\vx'_{s-1})[\vm_s,\vm_s]\\
    & = \Phi(\vx_0)  -\sum_{s=1}^k \eta_s\dotp{\nabla\Phi_{s-1}}{\vsigma_{s-1}} + \sum_{s=1}^k\frac{1}{2}\eta^2_s\nabla^2\Phi(\vx'_{s-1})[\vm_s,\vm_s]\\
    & +\mu_k\dotp{\nabla\Phi_{k-1}}{\vm_k}-\mu_1 \dotp{\nabla\Phi_{0}}{\vm_0} +\sum_{s=1}^{k-1}\mu_{s+1}\dotp{\nabla\Phi_{s-1}-\nabla\Phi_{s}}{\vm_{s}} + (\mu_s-\mu_{s+1})\dotp{\nabla\Phi_{s-1}}{\vm_{s}}\\
     & = \Phi(\vx_0)  -\sum_{s=1}^k \eta_s\dotp{\nabla\Phi_{s-1}}{\vsigma_{s-1}} + \sum_{s=1}^k\frac{1}{2}\eta^2_s\nabla^2\Phi(\vx'_{s-1})[\vm_s,\vm_s] +\mu_k\dotp{\nabla\Phi_{k-1}}{\vm_k}-\mu_1 \dotp{\nabla\Phi_{0}}{\vm_0}\\
    & +\sum_{s=1}^{k-1}[\mu_{s+1}\eta_s\nabla^2\Phi(\vx''_{s-1})[\vm_{s},\vm_{s}]+ (\mu_s-\mu_{s+1})\dotp{\nabla\Phi_{s-1}}{\vm_{s}}]
\end{align}

Let 
\begin{align}
  \vz_k = \vx_k - \Phi(\vx_k) + \Phi + \dots
\end{align}

and
\begin{align}
   Y_n = 
\end{align}

Then
\begin{align}
    \vx_a
\end{align}

When $\alpha\in (0,1)$, 
$\sum_{s=1}^{O(\eta^{-2})}\mu_{s+1}\eta_s\nabla^2\Phi(\vx''_{s-1})[\vm_{s},\vm_{s}] = O(1)$,
$\mu_k\dotp{\nabla\Phi_{k-1}}{\vm_k}=o(1)$


---------------------------

For SGD $\barvx_k = \barvx_{k-1} - \bareta_k \barvg_{k-1}$, the dynamics of $\Phi(\barvx_k)$ gives

\begin{align}
    \Phi(\barvx_k) - \Phi(\barvx_{k-1}) & = -\bareta_k\dotp{\nabla\Phi(\barvx_{k-1})}{\barvg_{k-1}} + \frac{1}{2}\bareta^2_k\nabla^2\Phi(\barvx')[\barvg_{k-1},\barvg_{k-1}]\\
\end{align}

compare with the dynamics of $\bvy_t$:
\[\dd\bvy_t = -\bareta_t \nabla\Phi(\bvy_t)\mSigma(\bvy_t)\dd W_t + \frac{1}{2} \bareta^2_t \nabla^2\Phi(\bvy_t)[\mSigma\mSigma^\top(\bvy_t)]\dd t \]

\begin{lemma}[Convergence to the Manifold]
    
\end{lemma}
\begin{lemma}[Averaging]
    For all $T>0$ and $l\in[d]$, 
    \begin{align}
        \E\sup_{}
    \end{align}
    
    
    
\end{lemma}

\fi