
\begin{theoremEnd}[category=complexityprojsgdqvc]{theorem}[\textbf{Strongly convex \(F\) with a decreasing stepsize schedule}]\label{thm:projsgd_stronglyconvex_decstepsize}
  For a \(\mu\)-strongly convex \(F : \Lambda \to \mathbb{R}\) on a convex set \(\Lambda\), the last iterate \(\vlambda_{T}\) of projected SGD with a descreasing stepsize satisfies \( {\lVert \vlambda_T - \vlambda^* \rVert}_2^2 \leq \epsilon \) if
  \begin{align*}
    \gamma_t = \min\left( \frac{\mu}{2 \alpha}, \frac{4 t + 2 }{ \mu \, {\left( t + 1\right)}^2 } \right)
    \quad\text{and}\quad 
    T \geq \frac{16 \beta}{ \mu^2 } \frac{1}{\epsilon} + \frac{8 \sqrt{2} \, \alpha \, \norm{\vlambda_0 - \vlambda^*}_2 }{ \mu^2} \frac{1}{\sqrt{\epsilon}}.
  \end{align*}
\end{theoremEnd}
\begin{proofEnd}
  Theorem 6 of \citet{domke_provable_2023} utilizes the two-stage stepsize of \citet{gower_sgd_2019}.
  After \(T\) steps, with a carefully tuned stepsize of 
  \[
    \gamma_t = \min\left( \frac{\mu}{2 \alpha}, \frac{4 t + 2 }{ \mu \, {\left( t + 1\right)}^2 } \right)
  \]
  the algorithm achieves
  \[
    \norm{\vlambda_{T} - \vlambda^*}_2^2
    \leq
    \frac{64 \alpha^2}{\mu^4} \frac{ \norm{\vlambda_0 - \vlambda^*}_2^2 }{T^2} 
    +
    \frac{32 \beta}{\mu^2} \frac{1}{T}.
  \]
  Following a similar strategy to \citet{kim_blackbox_2023}, we can obtain a computational complexity by solving for the smallest \(T\) that achieves
  \[
    \frac{64 \alpha}{\mu^2} \frac{ \norm{\vlambda_0 - \vlambda^*}_2^2 }{T^2} 
    +
    \frac{16 \beta}{\mu^2} \frac{1}{T}
    \leq
    \epsilon.
  \]
  After re-organizing, we solve for
  \[
     A \, T^2  + B \, T + C = 0,
  \]
  where 
  \[
    A = \epsilon, \quad
    B = -\frac{16 \beta}{\mu^2},\; \text{and} \quad
    C = - \frac{64 \alpha^2}{\mu^4} \norm{\vlambda_0 - \vlambda^*}_2^2.
  \]
  Since \(T > 0\), the equation has a unique root
  \begin{align*}
    T 
    &= \frac{ - B + \sqrt{ B^2 - 4 A C  } }{ 2 A },
\shortintertext{applying the inequality \(\sqrt{a + b} \leq \sqrt{a} + \sqrt{b}\) for \(a, b \geq 0\),}
    &\leq \frac{ - B + \sqrt{ B^2 } +  \sqrt{  4 A \left( -C \right)  } }{ 2 A }
    \\
    &= \frac{2 \left(-B\right) }{2 A} + \frac{ \sqrt{ 4 A  \left( -C \right)  } }{ 2 A }
    \\
    &= \frac{\left(-B\right)}{A} + \frac{ \sqrt{ 2 \left( -C \right) }  } { \sqrt{A} }
    \\
    &= \frac{ 16 \beta }{ \mu^2 \epsilon} + \frac{ \sqrt{  \frac{128\alpha^2}{\mu^4} \norm{\vlambda_0 - \vlambda^*}_2^2  }  } { \sqrt{\epsilon} }
    \\
    &= \frac{ 16 \beta }{ \mu^2 \epsilon} + \frac{ 8 \sqrt{2}  \alpha \norm{\vlambda_0 - \vlambda^*}_2 } { \mu^2 \sqrt{\epsilon} }.
  \end{align*}
\end{proofEnd}
