

\subsection{Proof of Lemma~\ref{lemma:opt}} \label{sec:proof-lemma:opt}
 %
 To begin with, we find it helpful to define the following function 
 %
 $$
	 f(p,v,n) \coloneqq \langle p, v\rangle + \max\Bigg\{\frac{20}{3}\sqrt{\frac{\mathbb{V}(p,v)\log \frac{1}{\delta'}} {n}} ,\frac{400}{9} \frac{H\log \frac{1}{\delta'}}{n} \Bigg\}
 $$ 
 %
 for any vector $p\in \Delta^{S}$, any non-negative vector $v\in \mathbb{R}^S$ obeying $\|v\|_{\infty}\leq H $, and any positive integer $n$. 
 We claim that 
%
\begin{equation}
	f(p,v,n)  \text{ is non-decreasing in each entry of }v.
	\label{eq:nondecreasing-f-property}
\end{equation}
% 
To justify this claim, consider any $1\leq s\leq S$, and let us freeze $p$, $n$ and all but the $s$-th entries of $v$.  
It then suffices to observe that (i) $f$ is a continuous function, and (ii) except for at most two possible choices of $v(s)$ that obey $\frac{20}{3}\sqrt{\frac{\mathbb{V}(p,v)\log \frac{1}{\delta'}} {n}}  =\frac{400}{9} \frac{H\log \frac{1}{\delta'}}{n} $, one can use the properties of $p$ and $v$ to calculate
	 %
 \begin{align}
	\frac{\partial f(p,v,n)}{\partial v(s)} & =p(s)+\frac{20}{3}\mathds{1}\Bigg\{\frac{20}{3}\sqrt{\frac{\mathbb{V}(p,v)\log\frac{1}{\delta'}}{n}}\geq\frac{400}{9}\frac{H\log\frac{1}{\delta'}}{n}\Bigg\}\frac{p(s)\big(v(s)-\langle p,v\rangle\big)\sqrt{\log\frac{1}{\delta'}}}{\sqrt{n\mathbb{V}(p,v)}}\nonumber\\
 & =p(s)+\mathds{1}\Bigg\{\sqrt{n\mathbb{V}(p,v)\log\frac{1}{\delta'}}\geq\frac{20}{3}H\log\frac{1}{\delta'}\Bigg\}\frac{\frac{20}{3}H\log\frac{1}{\delta'}}{\sqrt{n\mathbb{V}(p,v)\log\frac{1}{\delta'}}}\cdot\frac{p(s)\big(v(s)-\langle p,v\rangle\big)}{H}\nonumber\\
 & \geq\min\bigg\{ p(s)+p(s)\frac{\big(v(s)-\langle p,v\rangle\big)}{H},p(s)\bigg\}\nonumber\\
 & \geq p(s)\min\bigg\{\frac{H+v(s)-\langle p,v\rangle}{H},1\bigg\}\geq0,\nonumber
\end{align}
%
thus establishing the claim \eqref{eq:nondecreasing-f-property}. 


We now proceed to the proof of Lemma~\ref{lemma:opt}. 
	 Consider any $(h,k,s,a)$, and we divide into two cases. 

\paragraph{Case 1: $N_{h}^k(s,a) \leq 2$.}  
In this case, the following trivial bounds arise directly from the update rule \eqref{eq:update1}:  
%
$$
	 Q_h^k(s,a)=H \geq Q_h^{\star}(s,a) \qquad \text{and} \qquad V_h^k(s)=H\geq V_h^{\star}(s). 
$$ 
%


\paragraph{Case 2: $N_{h}^k(s,a) > 2$.}
%
Suppose now that $Q_{h+1}^k\geq Q_{h+1}^{\star}$, which also implies that $V_{h+1}^k \geq V_{h+1}^{\star}$. 
If $Q_h^k(s,a)=H$, then $Q_h^k(s,a)\geq Q_h^{\star}(s,a)$ holds trivially, 
and hence it suffices to look at the case with $Q_h^k(s,a)<H$. 
According to the update rule in \eqref{eq:update1}, it holds that
%
\begin{align}
 & Q_{h}^{k}(s,a)\nonumber\\
 & =\widehat{r}_{h}^{k}(s,a)+\big\langle\widehat{P}_{s,a,h}^{k},V_{h+1}^{k}\big\rangle\nonumber
 \\ & \qquad \qquad +c_{1}\sqrt{\frac{\mathbb{V}(\widehat{P}_{s,a,h}^{k},V_{h+1}^{k})\log\frac{1}{\delta'}}{N_{h}^{k}(s,a)}}+c_{2}\sqrt{\frac{\left(\widehat{\sigma}_{h}^{k}(s,a)-\big(\widehat{r}_{h}^{k}(s,a)\big)^{2}\right)\log\frac{1}{\delta'}}{N_{h}^{k}(s,a)}}+c_{3}\frac{H\log\frac{1}{\delta'}}{N_{h}^{k}(s,a)}\nonumber\\
 & \geq\widehat{r}_{h}^{k}(s,a)+2\sqrt{2}\sqrt{\frac{\left(\widehat{\sigma}_{h}^{k}(s,a)-\big(\widehat{r}_{h}^{k}(s,a)\big)^{2}\right)\log\frac{1}{\delta'}}{N_{h}^{k}(s,a)}}+\frac{48H\log\frac{1}{\delta'}}{3N_{h}^{k}(s,a)}+f\big(\widehat{P}_{s,a,h}^{k},V_{h+1}^{k},N_{h}^{k}(s,a)\big)\nonumber\\
 & \geq\widehat{r}_{h}^{k}(s,a)+2\sqrt{2}\sqrt{\frac{\left(\widehat{\sigma}_{h}^{k}(s,a)-\big(\widehat{r}_{h}^{k}(s,a)\big)^{2}\right)\log\frac{1}{\delta'}}{N_{h}^{k}(s,a)}}+\frac{48H\log\frac{1}{\delta'}}{3N_{h}^{k}(s,a)}+f\big(\widehat{P}_{s,a,h}^{k},V_{h+1}^{\star},N_{h}^{k}(s,a)\big)
	\label{eq:Qhk-sa-LB1}
% 
 \end{align}
%
for any $(s,a)$, where the last inequality results from the claim \eqref{eq:nondecreasing-f-property} and the property $V_{h+1}^k \geq V_{h+1}^{\star}$.
%
Moreover, applying Lemma \ref{empirical bernstein} and recalling the definition of $\widehat{\sigma}_h^k(s,a)$, we have 
%
\begin{subequations}
\label{eq_lemma1_ref.5+ref1}
%
\begin{align}
 & \mathbb{P}\left\{ \Big|\big\langle\widehat{P}_{s,a,h}^{k}-P_{s,a,h},\,V_{h+1}^{\star}\big\rangle\Big|>2\sqrt{\frac{\mathbb{V}\big(\widehat{P}_{s,a,h}^{k},V_{h+1}^{\star}\big)\log \frac{1}{\delta'}}{N_{h}^{k}(s,a)}}+\frac{14H\log \frac{1}{\delta'}}{3N_h^{k}(s,a)}\right\} \nonumber\\
 & \quad\leq\mathbb{P}\left\{ \Big|\big\langle\widehat{P}_{s,a,h}^{k}-P_{s,a,h},\,V_{h+1}^{\star}\big\rangle\Big|>\sqrt{\frac{2\mathbb{V}\big(\widehat{P}_{s,a,h}^{k},V_{h+1}^{\star}\big)\log \frac{1}{\delta'}}{N_{h}^{k}(s,a)-1}}+\frac{7H\log \frac{1}{\delta'}}{3N_{h}^{k}(s,a)-1}\right\} \leq2\delta'
	\label{eq_lemma1_ref.5}	
\end{align}
%
and
%
\begin{align}
\mathbb{P}\left\{ \Big|\widehat{r}_{h}^{k}(s,a)-r_{h}(s,a)\Big|>2\sqrt{\frac{\left(\widehat{\sigma}_{h}^{k}(s,a)-\big(\widehat{r}_{h}^{k}(s,a)\big)^{2}\right)\log \frac{1}{\delta'}}{N_{h}^{k}(s,a)}}+\frac{28H\log \frac{1}{\delta'}}{3N_{h}^{k}(s,a)}\right\}  & \leq2\delta' .
	\label{eq_lemma1_ref1}	
\end{align}
%
\end{subequations}
%
%where $\widehat{\mathrm{ Var}}_h^k(s,a) \leq \widehat{r}_h^k(s,a)$\footnote{ $\mathbb{E}\left[(Z-\mathbb{E}[Z])^2 \right]\leq  H\mathbb{E}\left[Z\right]$ for $Z\in [0,H]$.} is the empirical variance of $R_h(s,a)$ computed by the $N_h^k(s,a)$ samples.
%
These two inequalities imply that with probability exceeding $1-4\delta'$, 
%
\begin{align*}
r_{h}(s,a) & \leq\widehat{r}_{h}^{k}(s,a)+2\sqrt{2}\sqrt{\frac{\left(\widehat{\sigma}_{h}^{k}(s,a)-\big(\widehat{r}_{h}^{k}(s,a)\big)^{2}\right)\log\frac{1}{\delta'}}{N_{h}^{k}(s,a)}}+\frac{28H\log\frac{1}{\delta'}}{3N_{h}^{k}(s,a)};\\
f\big(\widehat{P}_{s,a,h}^{k},V_{h+1}^{\star},N_{h}^{k}(s,a)\big) & =\big\langle P_{s,a,h},V_{h+1}^{\star}\big\rangle+\big\langle\widehat{P}_{s,a,h}^{k}-P_{s,a,h},V_{h+1}^{\star}\big\rangle\\
 & \qquad+\max\Bigg\{\frac{20}{3}\sqrt{\frac{\mathbb{V}(\widehat{P}_{s,a,h}^{k},V_{h+1}^{\star})\log\frac{1}{\delta'}}{N_{h}^{k}(s,a)}},\frac{400}{9}\frac{H\log\frac{1}{\delta'}}{N_{h}^{k}(s,a)}\Bigg\}\\
 & \geq\big\langle P_{s,a,h},V_{h+1}^{\star}\big\rangle.
\end{align*}
%
Substitution into \eqref{eq:Qhk-sa-LB1} gives: with probability at least $1-4\delta'$,  
$$	
Q_h^k(s,a)\geq r_h(s,a)+ \big\langle P_{s,a,h}, V_{h+1}^{\star} \big\rangle= Q_h^{\star}(s,a).
$$
%


\paragraph{Putting all this together.} 
%
With the above two cases in place,  one can invoke standard induction arguments to deduce that: with probability at least $1-4SAHK\delta'$, one has $Q_h^k(s,a)\geq Q_h^{\star}(s,a)$ 
and $V_h^k = \max_a Q_h^k(s,a)\geq \max_a Q_h^{\star}(s,a)= V_h^{\star}(s)$ for every $(s,a,h,k)$. The proof is thus completed.
%
%Via a union bound over all $(s,a)$ and $i$, we obtain that $\mathbb{P}\left[\mathcal{E}_1\cap \mathcal{E}_2\right]\geq 1 -2SA(\log_{2}KH+1)\delta$. The proof is completed.
%
%On the other hand, using empirical Bernstein's inequality,  we can verify that $f(\widehat{P}_{s,a,h}^k, V_{h+1}^{\star}, N_{s,a,h}^k)\geq Q_{h}^{\star}(s,a)$ with probability $1-2\delta$. With a union bound on the failure probability, we obtain that with probability $1-2SAHK\delta$, $Q_h^k(s,a)\geq Q_h^{\star}(s,a)$  and $V^k_h(s)\geq V^{\star}_h(s)$ for any proper $(s,a,h,k)$. 
% \end{proof}










\subsection{Proof of Lemma~\ref{lem:bound-T234}}\label{app:pflem:bound-T234}

\subsubsection{Bounding $T_2$} 
%
We first establish the bound \eqref{eq:boundt2} on $T_2$. To begin with, $T_2$ can be decomposed using the definition \eqref{eq:update1} of the bonus term:  
%
\begin{align}
T_{2} & =\sum_{k=1}^{K}\sum_{h=1}^{H}b_{h}^{k}(s_{h}^{k},a_{h}^{k})\nonumber\\
 & =\frac{460}{9}\sum_{k,h}\sqrt{\frac{\mathbb{V}\big(\widehat{P}_{s_{h}^{k},a_{h}^{k},h}^{k},V_{h+1}^{k}\big)\log\frac{1}{\delta'}}{N_{h}^{k}(s_{h}^{k},a_{h}^{k})}}+2\sqrt{2}\sum_{k,h}\sqrt{\frac{\left(\widehat{\sigma}_{h}^{k}(s_{h}^{k},a_{h}^{k})-\big(\widehat{r}_{h}^{k}(s_{h}^{k},a_{h}^{k})\big)^{2}\right)\log\frac{1}{\delta'}}{N_{h}^{k}(s_{h}^{k},a_{h}^{k})}}\nonumber\\
 & \qquad\qquad\qquad\qquad\qquad\qquad\qquad\qquad\qquad\qquad\qquad\qquad+\frac{544}{9}\sum_{k,h}\frac{H\log\frac{1}{\delta'}}{N_{h}^{k}(s_{h}^{k},a_{h}^{k})}.
	\label{eq:T2-decomposition-main1}
\end{align}
%
Applying the Cauchy-Schwarz inequality and invoking Lemma~\ref{lemma:doubling}, we obtain
%
\begin{align}
T_{2} & \leq\frac{460}{9}\sqrt{\sum_{k,h}\frac{\log\frac{1}{\delta'}}{N_{h}^{k}(s_{h}^{k},a_{h}^{k})}}\sqrt{\sum_{k,h}\mathbb{V}\big(\widehat{P}_{s_{h}^{k},a_{h}^{k},h}^{k},V_{h+1}^{k}\big)}\nonumber\\
 & \qquad+2\sqrt{2}\sqrt{\sum_{k,h}\frac{\log\frac{1}{\delta'}}{N_{h}^{k}(s_{h}^{k},a_{h}^{k})}}\sqrt{\sum_{k,h}\left(\widehat{\sigma}_{h}^{k}(s_{h}^{k},a_{h}^{k})-\big(\widehat{r}_{h}^{k}(s_{h}^{k},a_{h}^{k})\big)^{2}\right)}+\frac{544H\log\frac{1}{\delta'}}{9}\sum_{k,h}\frac{1}{N_{h}^{k}(s_{h}^{k},a_{h}^{k})}\nonumber\\
 & \leq\frac{460}{9}\sqrt{2SAH(\log_{2}K)\Big(\log\frac{1}{\delta'}\Big)\sum_{k,h}\mathbb{V}\big(\widehat{P}_{s_{h}^{k},a_{h}^{k},h}^{k},V_{h+1}^{k}\big)}\nonumber\\
 & \qquad+4\sqrt{SAH(\log_{2}K)\log\frac{1}{\delta'}}\sqrt{\sum_{k,h}\left(\widehat{\sigma}_{h}^{k}(s_{h}^{k},a_{h}^{k})-\big(\widehat{r}_{h}^{k}(s_{h}^{k},a_{h}^{k})\big)^{2}\right)}+\frac{1088}{9}SAH^{2}(\log_{2}K)\log\frac{1}{\delta'}.
	\label{eq:boundt2o-temp}
\end{align}
%
Using the basic fact $\widehat{\sigma}_h^k(s_h^k,a_h^k) \leq H\widehat{r}_h^k(s,a)$ (since each immediate reward is at most $H$) and the definition \eqref{eq:defn-T5-proof} of $T_5$,  we can continue the bound in \eqref{eq:boundt2o-temp} to derive
%
\begin{align}
T_{2} & \leq\frac{460}{9}\sqrt{2SAH(\log_{2}K)\Big(\log\frac{1}{\delta'}\Big)T_{5}}\nonumber\\
 & \qquad+4\sqrt{SAH^{2}(\log_{2}K)\log\frac{1}{\delta'}}\sqrt{\sum_{k,h}\widehat{r}_{h}^{k}(s_{h}^{k},a_{h}^{k})}+\frac{1088}{9}SAH^{2}(\log_{2}K)\log\frac{1}{\delta'}.
	\label{eq:boundt2o}
\end{align}
%
%where we define $T_5 = \sum_{k=1}^K\sum_{h=1}^H\mathbb{V}(\widehat{P}^k_{s_h^k,a_h^k,h},V_{h+1}^k )$, and the last inequality is by the fact that $\left(\widehat{\sigma}_h^k(s_h^k,a_h^k)- (\widehat{r}_h^k(s_h^k,a_h^k))^2\right)\leq H\widehat{r}_h^k(s,a)$ for any proper $(s,a,h,k)$. 
%
Applying Lemma~\ref{lemma:bdempr} to bound $\sum_{k,h}\widehat{r}_h^k(s_h^k,a_h^k)$ 
and using the basic fact $\sum_{k,h} r_h(s_h^k,a_h^k)\leq KH$, 
we can employ a little algebra to deduce that 
%
\begin{align*}
	T_2\leq 61\sqrt{2SAH(\log_2 K)\Big(\log\frac{1}{\delta'}\Big)T_5} +  8\sqrt{SAH^3K(\log_2 K)\log\frac{1}{\delta'}}+
	155SAH^2(\log_2K)\log\frac{1}{\delta'}
	%\label{eq:boundt2}
\end{align*}
%
with probability exceeding $1-2SAHK\delta'$. 



%\noindent 
%Taking Lemma~\ref{lemma:bdempr} together with the basic fact $\sum_{k,h} r_h(s_h^k,a_h^k)\leq KH$, we arrive at
%%
%\begin{align}
%	\left| \sum_{k=1}^{K}\sum_{h=1}^{H} \Big( \widehat{r}_{h}^{k}(s_{h}^{k},a_{h}^{k})-r_{h}(s_{h}^{k},a_{h}^{k}) \Big)\right| 
%	&\leq \sum_{k=1}^{K}\sum_{h=1}^{H}\left|\widehat{r}_{h}^{k}(s_{h}^{k},a_{h}^{k})-r_{h}(s_{h}^{k},a_{h}^{k})\right| \notag\\
%	%&\leq4SAH^{2}+4\sqrt{2SAH^{3}K(\log_{2}K)\log\frac{1}{\delta'}}+48SAH^{2}(\log_{2}K)\log\frac{1}{\delta'} \nonumber\\
%	&\leq 4\sqrt{2SAH^{3}K(\log_{2}K)\log\frac{1}{\delta'}}+52SAH^{2}(\log_{2}K)\log\frac{1}{\delta'}.
%	\label{eq:sum-rhat-sum-r-diff}
%\end{align}
%


\subsubsection{Bounding $T_3$} 
%
Next, let us prove the bound \eqref{eq:boundt3} on $|T_3|$. 
Recall that $V_{h+1}^{k}(s)$ denotes the value function estimate
of state $s$ \emph{before} the $k$-th episode, which corresponds
to the value estimate computed at the end of the \emph{previous epoch}.
This important fact implies that conditional on  $(s_{h}^{k},a_{h}^{k})$, the vector $e_{s_{h+1}^{k}}$ is statistically independent of $V_{h+1}^{k}$ and has conditional mean $P_{s_{h}^{k},a_{h}^{k},h}$,  
allowing us to invoke the Freedman inequality for
martingales (see Lemma~\ref{lemma:self-norm}) to control the sum
of $\big\langle P_{s_{h}^{k},a_{h}^{k},h}-e_{s_{h+1}^{k}},V_{h+1}^{k}\big\rangle$. 
Recalling the definition of $T_6$ in \eqref{eq:defn-T6-proof}, 
we can see from Lemma~\ref{lemma:self-norm} that
%
\begin{align}
 |T_3|  \leq 2\sqrt{2}\cdot \sqrt{  T_6 \log \frac{1}{\delta'} } + \log \frac{1}{\delta'} + 2H\log \frac{1}{\delta'} 
	\leq 2\sqrt{2}\cdot \sqrt{  T_6 \log \frac{1}{\delta'}  } + 3H\log \frac{1}{\delta'} \label{eq:boundt3-proof}
\end{align}
%
with probability at least $1-10SAH^2K^2\delta'$. 
 





\subsubsection{Bounding $T_4$} 
%
We now turn attention to the bound \eqref{eq:bdt_4f} on $|T_4|$. 
Recall that
%
\begin{align}
T_4 = \sum_{k=1}^K\sum_{h=1}^H \left(\widehat{r}_h^k(s_h^k,a_h^k) - r_h(s_h^k,a_h^k)  \right) + \sum_{k=1}^K \left( \sum_{h=1}^H r_h(s_h^k,a_h^k) - V_1^{\pi^k}(s_1^k) \right),
	\label{eq:T4-defn-repeat}
\end{align}
%
and we shall bound the two terms above separately. 
%
\begin{itemize}
	\item Regarding the first term on the right-hand side of \eqref{eq:T4-defn-repeat}, we can apply Lemma~\ref{lemma:bdempr} and the fact $\sum_{k,h} r_h(s_h^k,a_h^k)\leq KH$ to show that
%can apply  Lemma~\ref{lemma:bdempr} and use the fact $\sum_{k,h} r_h(s_h^k,a_h^k)\leq KH$ to obtain
%
\begin{align}
  \left| \sum_{k=1}^K\sum_{h=1}^H \big(\widehat{r}_h^k(s_h^k,a_h^k)-r_{h}(s_h^k,a_h^k)\big)\right|
%\\ & \leq 4SAH^2 +4\sqrt{2\log_2(K)SAH^2}\cdot \sqrt{KH} + 24\log_2(K)SAH^2\log(\frac{1}{\delta'})\nonumber
%\\ & 
	\leq  4\sqrt{2SAH^3K (\log_2K)\log\frac{1}{\delta'}}+52 SAH^2 (\log_2K)\log \frac{1}{\delta'}\label{eq:bdt4_2}
\end{align}
%
holds with probability at least $1-2SAHK\delta'$. 
	\item
With regards to the second term on the right-hand side of \eqref{eq:T4-defn-repeat}, 
we note that conditional on $\pi^k$,  $E_k:=\sum_{h=1}^H r_{h}(s_h^k,a_h^k)- V_1^{\pi^k}(s_1^k)$ is a zero-mean random variable bounded in magnitude by $H$. 
According to Lemma~\ref{lemma:self-norm}, 
\begin{align}
	\left| \sum_{k=1}^K E_k \right|
	&\leq 2\sqrt{2}\cdot \sqrt{\sum_{k=1}^K \mathsf{Var}(E_k)\log \frac{1}{\delta'} } + 3H^2\log \frac{1}{\delta'} \nonumber\\
	&\leq 2\sqrt{2KH^2\log \frac{1}{\delta'}} + 3H^2 \log \frac{1}{\delta'}
	\label{eq:bdt4_1}
\end{align}
%
holds with probability exceeding $1- 4\delta' \log_2(KH)$, 
where $\mathsf{Var}(E_k)$ denotes the variance of $E_k$  conditioned on what happens before the $k$-th episode, 
and the last inequality follows since $|E_k|\leq H$ always holds. 
%
\end{itemize}

Substituting \eqref{eq:bdt4_2} and \eqref{eq:bdt4_1} into \eqref{eq:T4-defn-repeat} reveals that with probability at least $1-3SAHK\delta'$, 
%
\begin{align}
	|T_4| \leq 6\sqrt{2SAH^3K(\log_2K)\log \frac{1}{\delta'} } +  55SAH^2(\log_2 K)\log \frac{1}{\delta'}.\label{eq:bdt_4f-proof}
\end{align}






\subsection{Proof of Lemma~\ref{lem:bound-T56}} \label{sec:pflem:bound-T56}
%
Regarding the term $T_5$, direct calculation gives 
%
\begin{align}
T_{5} & =\sum_{k=1}^{K}\sum_{h=1}^{H}\mathbb{V}\big(\widehat{P}_{s_{h}^{k},a_{h}^{k},h}^{k},V_{h+1}^{k}\big)=\sum_{k=1}^{K}\sum_{h=1}^{H}\left(\Big\langle\widehat{P}_{s_{h}^{k},a_{h}^{k},h}^{k},\big(V_{h+1}^{k}\big)^{2}\Big\rangle-\big(\big\langle\widehat{P}_{s_{h}^{k},a_{h}^{k},h}^{k},V_{h+1}^{k}\big\rangle\big)^{2}\right)\nonumber\\
 & =\underset{=\:T_{7}}{\underbrace{\sum_{k=1}^{K}\sum_{h=1}^{H}\Big\langle\widehat{P}_{s_{h}^{k},a_{h}^{k},h}^{k}-P_{s_{h}^{k},a_{h}^{k},h},\big(V_{h+1}^{k}\big)^{2}\Big\rangle}}+\underset{=\:T_{8}}{\underbrace{\sum_{k=1}^{K}\sum_{h=1}^{H}\Big\langle P_{s_{h}^{k},a_{h}^{k},h}-e_{s_{h+1}^{k}},\big(V_{h+1}^{k}\big)^{2}\Big\rangle}}\nonumber\\
 & \qquad\qquad\qquad\qquad\qquad\qquad+\sum_{k=1}^{K}\sum_{h=1}^{H}\big(V_{h+1}^{k}(s_{h+1}^{k})\big)^{2}-\sum_{k=1}^{K}\sum_{h=1}^{H}\big(\big\langle\widehat{P}_{s_{h}^{k},a_{h}^{k},h}^{k},V_{h+1}^{k}\big\rangle\big)^{2}\notag\\
 & =T_{7}+T_{8}+\sum_{k=1}^{K}\sum_{h=2}^{H}\big(V_{h}^{k}(s_{h}^{k})\big)^{2}-\sum_{k=1}^{K}\sum_{h=1}^{H}\big(\big\langle\widehat{P}_{s_{h}^{k},a_{h}^{k},h}^{k},V_{h+1}^{k}\big\rangle\big)^{2}\notag\\
 & \leq T_{7}+T_{8}+2H\sum_{k=1}^{K}\sum_{h=1}^{H}\max\Big\{ V_{h}^{k}(s_{h}^{k})-\big\langle\widehat{P}_{s_{h}^{k},a_{h}^{k},h}^{k},V_{h+1}^{k}\big\rangle,0\Big\}\nonumber\\
 & \leq T_{7}+T_{8}+2H\sum_{k=1}^{K}\sum_{h=1}^{H}b_{h}^{k}(s_{h}^{k},a_{h}^{k})+2H\sum_{k=1}^{K}\sum_{h=1}^{H}\widehat{r}^k_{h}(s_{h}^{k},a_{h}^{k})\label{eq:boundt5-intermediate-13}\\
 & \leq T_{7}+T_{8}+2HT_{2}+6KH^{2}\label{eq:boundt5-intermediate}
\end{align}
%
with probability at least $1-3\delta'\log(KH^{3})$. Here, the third line utilizes the fact that $V_{H+1}^k=0$,  
the first inequality holds since 
%
\begin{align*}
\big(V_{h}^{k}(s_{h}^{k})\big)^{2}-\big(\big\langle\widehat{P}_{s_{h}^{k},a_{h}^{k},h}^{k},V_{h+1}^{k}\big\rangle\big)^{2} 
	& =\Big(V_{h}^{k}(s_{h}^{k})+\big\langle\widehat{P}_{s_{h}^{k},a_{h}^{k},h}^{k},V_{h+1}^{k}\big\rangle\Big)\Big(V_{h}^{k}(s_{h}^{k})-\big\langle\widehat{P}_{s_{h}^{k},a_{h}^{k},h}^{k},V_{h+1}^{k}\big\rangle\Big)\\
 & \leq2H\max\left\{ V_{h}^{k}(s_{h}^{k})-\big\langle\widehat{P}_{s_{h}^{k},a_{h}^{k},h}^{k},V_{h+1}^{k}\big\rangle,\,0\right\} ,
\end{align*}
%
 the penultimate line makes use of the property $V_{h}^{k}(s_{h}^{k})=Q_{h}^{k}(s_{h}^{k},a_{h}^{k})$ and the update rule \eqref{eq:updateq}, 
 whereas the last line applies property \eqref{eq:sum-empirical-r-UB} and the definition \eqref{eq:boundt2} of $T_2$. 



%Let $T_7  =  \sum_{k=1}^K \sum_{h=1}^H   (\widehat{P}^k_{s_h^k,a_h^k,h} -P_{s_h^k,a_h^k,h})(V^k_{h+1})^2  $ and $T_8 = \sum_{k=1}^K \sum_{h=1}^H (P_{s_h^k,a_h^k,h} - \textbf{1}_{s_{h+1}^k} )  (V_{h+1}^k)^2$.

Akin to the above bound on $T_5$, we can show that with probability at least $1-3SAHK\delta'$, 
%
\begin{align}
T_{6} & =\sum_{k=1}^{K}\sum_{h=1}^{H}\mathbb{V}\big(P_{s_{h}^{k},a_{h}^{k},h},V_{h+1}^{k}\big)=\sum_{k=1}^{K}\sum_{h=1}^{H}\Big\langle P_{s_{h}^{k},a_{h}^{k},h},\big(V_{h+1}^{k}\big)^{2}\Big\rangle-\sum_{k=1}^{K}\sum_{h=1}^{H}\Big(\big\langle P_{s_{h}^{k},a_{h}^{k},h},V_{h+1}^{k}\big\rangle\Big)^{2}\nonumber\\
 & =\sum_{k=1}^{K}\sum_{h=1}^{H}\Big\langle P_{s_{h}^{k},a_{h}^{k},h}-e_{s_{h+1}^{k}},\big(V_{h+1}^{k}\big)^{2}\Big\rangle+\sum_{k=1}^{K}\sum_{h=2}^{H}\big(V_{h}^{k}(s_{h}^{k})\big)^{2}-\sum_{k=1}^{K}\sum_{h=1}^{H}\Big(\big\langle P_{s_{h}^{k},a_{h}^{k},h},V_{h+1}^{k}\big\rangle\Big)^{2}\nonumber\\
 & \leq T_{8}+2H\sum_{k=1}^{K}\sum_{h=1}^{H}\max\Big\{ V_{h}^{k}(s_{h}^{k})-\big\langle P_{s_{h}^{k},a_{h}^{k},h},V_{h+1}^{k}\big\rangle,0\Big\}\notag\\
 & \leq T_{8}+2H\sum_{k=1}^{K}\sum_{h=1}^{H}\max\Big\{ V_{h}^{k}(s_{h}^{k})-\big\langle\widehat{P}_{s_{h}^{k},a_{h}^{k},h},V_{h+1}^{k}\big\rangle,0\Big\}+2H\sum_{k=1}^{K}\sum_{h=1}^{H}\max\Big\{\big\langle\widehat{P}_{s_{h}^{k},a_{h}^{k},h}^{k}-P_{s_{h}^{k},a_{h}^{k},h},V_{h+1}^{k}\big\rangle,0\Big\}\nonumber\\
 & \leq T_{8}+2H\sum_{k=1}^{K}\sum_{h=1}^{H}b_{h}^{k}(s_{h}^{k},a_{h}^{k})+2H\sum_{k=1}^{K}\sum_{h=1}^{H}\widehat{r}_{h}^{k}(s_{h}^{k},a_{h}^{k})+2HT_{9}\label{eq:boundt6-intermediate-135}\\
 & \leq T_{8}+2HT_{2}+6KH^2+2HT_{9}.\label{eq:boundt6-intermediate}
\end{align}
%
%where we recall the definition of $T_2$ in \eqref{eq:boundt2} and have applied property \eqref{eq:sum-empirical-r-UB} in the last line. 
%



%Let $T_9 = \sum_{k=1}^K \sum_{h=1}^H \max\{ (\widehat{P}^k_{s_h^k,a_h^k,h} - P_{s_h^k,a_h^k,h})V_{h+1}^k,0 \}$.




Finally, note that the above bounds on $T_5$ and $T_6$ both depend on the term $T_8$ (cf.~\eqref{eq:defn-T8-proof}), 
which we would like to cope with now. 
%
Using Freedman's inequality (cf.~Lemma~\ref{lemma:self-norm}) and the fact that $\mathsf{Var}(X^2)\leq 4 H^2\mathsf{Var}(X)$ for any random variable $X$ with support on $[-H,H]$ (cf.~Lemma~\ref{lemma:sqv}), we reach
%
\begin{align}
	|T_{8}|\leq2\sqrt{2}\sqrt{\sum_{k,h}\mathbb{V}\Big(\widehat{P}_{s_{h}^{k},a_{h}^{k},h}^{k},\big(V_{h+1}^{k}\big)^{2}\Big)\log\frac{1}{\delta'}}+3H^{2}\log\frac{1}{\delta'}\leq \sqrt{32H^{2}T_{6}\log\frac{1}{\delta'}}+3H^{2}\log\frac{1}{\delta'}	 
	%\label{eq:boundt8}
\end{align}
%
with probability at least $1-3\delta'\log(KH^{3})$. 
Substitution into \eqref{eq:boundt5-intermediate} and \eqref{eq:boundt6-intermediate} establishes \eqref{eq:boundt56}. 
%
%Putting the preceding bounds together yields
%%
%\begin{subequations}
%\begin{align}
%T_{5} & \leq T_{7}+2HT_{2}+6KH^{2}+\sqrt{32H^{2}T_{6}\log\frac{1}{\delta'}}+3H^{2}\log\frac{1}{\delta'} 
%\label{eq:boundt5-temp} \\
%T_{6} & \leq2HT_{2}+6KH^{2}+\sqrt{32H^{2}T_{6}\log\frac{1}{\delta'}}+3H^{2}\log\frac{1}{\delta'}+2HT_{9}
%\label{eq:boundt6-temp}
%\end{align}
%\end{subequations}
%%
%with probability at least $1-4SAHK\delta'$. 
%
%\end{proof}

