

\section{Technical Lemmas}
This section is dedicated to presenting several lemmas that serve as building blocks in proving the convergence of our proposed algorithms.



\begin{lemma}[Perturbed strong convexity, \citet{karimireddy2020scaffold}]\label{lemma:perturb-strong-convexity}
Suppose the function $f(\cdot): \mathcal{X} \rightarrow \mathbb{R}$ is $L$-smooth and $\mu$-strongly convex, then for any $\bx, \by, \bz \in \mathcal{X}$,
\begin{equation}
    \langle \nabla f(\bx), \bz -\by \rangle \geq f(\bz) - f(\by) + \frac{\mu}{4}\|\by - \bz\|^{2} - L\|\bz - \bz\|^{2}.
\end{equation}
\end{lemma}


We now present the lemma for analyzing the drift term.
\begin{lemma}[Bounded drift]\label{Lemma:drift-lemma-deterministic}
Suppose $\tau_r = J\,\eta_{\ell}\,\eta_{g}$, and $\eta_{g}\geq 1$, then we have
\begin{equation}
    \mathcal{E}_{r} \leq \frac{12\tau^{2}}{\eta_{g}^{2}}\E\left[\left\|\nabla_{\bx} \Phi(\bx^{r}, \blambda^{r+1})\right\|^{2}\right] + \frac{12\tau^{2}}{\eta_{g}^{2}}\left(1+\chi\right)\zeta^{2} + \frac{3\tau^{2}}{\eta_g^{2} J}\zeta^{2},
\end{equation}
where $\mathcal{E}_r$ is defined as
\begin{equation}
\mathcal{E}_{r} = \frac{1}{J}\sum_{i=1}^{N}\sum_{j=1}^{J}\lambda_{i}\E\left[\|\bu_{i, j} - \bx\|^{2}\right],
\end{equation}
and $\chi$ is defined as
\begin{equation}
    \chi = \max_{\blambda \in \Lambda} \sum_{i=1}^{N}\lambda_i^{2}.
\end{equation}
\end{lemma}

\begin{proof}
We omit the $r$ superscript in the following proof. 
Recall that the definition of $\bu_{i,j}$ in Algorithm~\ref{Algorithm:ScaffoldAPD}, i.e.,
$$\bu_{i,j}=\bu_{i,j-1} - \eta_{\ell}\left(g_i(\bu_{i,j-1}) - \hat{\bc}_i + \hat{\bc}\right),$$ 
and we have
\begin{equation}
\begin{aligned}
    \E\left[g_i(\bu_{i,j-1})\right] &= \nabla f_i(\bu_{i,j-1}),\\
    \E\left[\hat{\bc}_i\right] &= \nabla f_i(\bx) = \bc_i,\\
    \E\left[\hat{\bc}\right] &=  
    \sum_{i=1}^{N}\lambda_i \nabla f_i(\bx) = \bc.
\end{aligned}
\end{equation}
Then we can upper bound $\E\left[\|\bu_{i, j} - \bx\|^{2}\right]$ as follows,
\begin{equation}
\begin{aligned}
&\E\left[\|\bu_{i, j} - \bx\|^{2}\right] \\
=\,& \E\left[\|\bu_{i, j-1} - \bx - \eta_{\ell}( g_i(\bu_{i,j-1})- \hat{\bc_i} + \hat{\bc})\|^{2}\right]\\
=\,& \E\left[\|\bu_{i, j-1} - \bx - \eta_{\ell}( \nabla f_i(\bu_{i,j-1})- \hat{\bc_i} + \hat{\bc})\|^{2}\right] + \eta_{\ell}^{2}\E\left[\| g_i(\bu_{i,j-1}) - \nabla f_i(\bu_{i,j-1})\|^{2}\right]\\
\leq\,& \E\left[\|\bu_{i, j-1} - \bx - \eta_{\ell}( \nabla f_i(\bu_{i,j-1})- \hat{\bc_i} + \hat{\bc})\|^{2}\right] + \eta_{\ell}^{2}\zeta^{2}\\
\leq\,& \left(1 + \frac{1}{J-1}\right)\E\left[\|\bu_{i, j-1} - \bx \|^{2}\right] + J\eta_{\ell}^{2}\E\left[\|\nabla f_i(\bu_{i,j-1})- \hat{\bc}_i + \hat{\bc}\|^{2}\right] + \eta_{\ell}^{2}\zeta^{2}\\
=\,& \left(1 + \frac{1}{J-1}\right)\E\left[\|\bu_{i, j-1} - \bx \|^{2}\right] + \frac{\tau^{2}}{\eta_{g}^{2}J}\E\left[\|\nabla f_i(\bu_{i,j-1})- \hat{\bc}_i + \hat{\bc}\|^{2}\right] + \eta_{\ell}^{2}\zeta^{2} \\
\leq\,& \left(1 + \frac{1}{J-1}\right)\E\left[\|\bu_{i, j-1} - \bx \|^{2}\right] + \frac{2\tau^{2}}{\eta_{g}^{2}J}\E\left[\|\nabla f_i(\bu_{i,j-1})- {\bc}_i + {\bc}\|^{2}\right]  \\
& \quad + \frac{2\tau^{2}}{\eta_{g}^{2}J}\E\left[\|\hat{\bc}_i -  {\bc}_i + {\bc} - \hat{\bc}\|^{2}\right]+ \eta_{\ell}^{2}\zeta^{2} \\
\leq\,& \left(1 + \frac{1}{J-1}\right)\E\left[\|\bu_{i, j-1} - \bx \|^{2}\right] + \frac{2\tau^{2}}{\eta_{g}^{2}J}\E\left[\|\nabla f_i(\bu_{i,j-1})- {\bc}_i + {\bc}\|^{2}\right]  \\
& \quad + 
\underbrace{\frac{4\tau^{2}}{\eta_{g}^{2}J}\E\left[\|\hat{\bc}_i -  {\bc}_i\|^{2}\right] + \frac{4\tau^{2}}{\eta_{g}^{2}J}\E\left[\| \hat{\bc} - {\bc}\|^{2}\right] + \eta_{\ell}^{2}\zeta^{2}}_{ \Gamma},
\end{aligned}
\end{equation}
where $\Gamma = 0$ if the local gradients are deterministic. Next, we could first upper bound the term $\E\left[\|\bu_{i, j} - \bx\|^{2}\right]$ as 
\begin{equation}
\begin{aligned}
&\E\left[\|\bu_{i, j} - \bx\|^{2}\right] \\
\leq\,& \left(1 + \frac{1}{J-1}\right)\E\left[\|\bu_{i, j-1} - \bx \|^{2}\right] + \frac{4\tau^{2}}{\eta_{g}^{2}J}\E\left[\|\nabla f_i(\bu_{i,j-1})- \bc_i\|^{2}\right]+ \frac{4\tau^{2}}{\eta_{g}^{2}J}\E\left[\| \bc\|^{2}\right] + \Gamma\\
\leq\,& \left(1 + \frac{1}{J-1}+\frac{4\tau^{2}L_{\bx\bx}^{2}}{\eta_{g}^{2}J}\right)\E\left[\|\bu_{i, j-1} - \bx \|^{2}\right] + \frac{4\tau^{2}}{\eta_{g}^{2}J}\E\left[\| \bc\|^{2}\right] + \Gamma \\
\leq\,& \left(1 + \frac{2}{J-1}\right)\E\left[\|\bu_{i, j-1} - \bx \|^{2}\right]  + \frac{4\tau^{2}}{\eta_{g}^{2}J}\E\left[\| \bc\|^{2}\right] + \Gamma ,
\end{aligned}
\end{equation}
where we apply the condition that $\frac{4\tau^{2}L_{\bx\bx}^{2}}{\eta_{g}^{2}J} \leq \frac{1}{J-1}$. Then we have
\begin{equation}
\begin{aligned}
    \E\left[\|\bu_{i, j} - \bx\|^{2}\right] 
    &\leq \sum_{i=1}^{j-1} \left(1 + \frac{2}{J-1}\right)^{i} \left(\frac{4\tau^{2}}{\eta_{g}^{2}J}\E\left[\| \bc\|^{2}\right] + \Gamma \right) \\
    &\leq 3J \left(\frac{4\tau^{2}}{\eta_{g}^{2}J}\E\left[\| \bc\|^{2}\right] + \Gamma \right)
    = \frac{12\tau^{2}}{\eta_{g}^{2}}\E\left[\| \bc\|^{2}\right] + 3J\,\Gamma.
\end{aligned}
\end{equation}
Then the drift error $\mathcal{E}_{r}$ can be upper bounded  as follows,
\begin{equation*}
\begin{aligned}
    \mathcal{E}_{r} & = \frac{1}{J}\sum_{i=1}^{N}\sum_{j=1}^{J}\lambda_{i}\E\left[\|\bu_{i, j} - \bx\|^{2}\right] \\
    &\leq \frac{1}{J}\sum_{i=1}^{N}\sum_{j=1}^{J}\lambda_i \frac{12\tau^{2}}{\eta_{g}^{2}}\E\left[\| \bc\|^{2}\right] + \frac{1}{J}\sum_{i=1}^{N}\sum_{j=1}^{J}3\lambda_i J\,\Gamma \\
    &=  \frac{12\tau^{2}}{\eta_{g}^{2}}\E\left[\Big\|\sum_{i=1}^{N}\lambda_{i}\nabla f_i(\bx)\Big\|^{2}\right] + 3J\cdot\left(\frac{4\tau^{2}}{\eta_{g}^{2}J}\sum_{i=1}^{N}\lambda_i\E\left[\|\hat{\bc}_i -  {\bc}_i\|^{2}\right] + \frac{4\tau^{2}}{\eta_{g}^{2}J}\E\left[\| \hat{\bc} - {\bc}\|^{2}\right] + \eta_{\ell}^{2}\zeta^{2}\right) \\
    &\leq  \frac{12\tau^{2}}{\eta_{g}^{2}}\E\left[\Big\|\sum_{i=1}^{N}\lambda_{i}\nabla f_i(\bx)\Big\|^{2}\right] + \left(\frac{12\tau^{2}}{\eta_{g}^{2}}\sum_{i=1}^{N}\lambda_i \E\left[\|\hat{\bc}_i -  {\bc}_i\|^{2}\right] + \frac{12\tau^{2}}{\eta_{g}^{2}}\E\left[\| \hat{\bc} - {\bc}\|^{2}\right] + \frac{3\tau^{2}}{\eta_g^{2} J}\zeta^{2}\right) \\
    &\leq  \frac{12\tau^{2}}{\eta_{g}^{2}}\E\left[\left\|\nabla_{\bx} \Phi(\bx, \blambda)\right\|^{2}\right] + \frac{12\tau^{2}}{\eta_{g}^{2}}\zeta^{2} +  \frac{12\tau^{2}}{\eta_{g}^{2}}\underbrace{\left(\sum_{i=1}^{N}\lambda_i^{2} \right)}_{\leq \chi}\zeta^{2} + \frac{3\tau^{2}}{\eta_g^{2} J}\zeta^{2}\\
    &\leq  \frac{12\tau^{2}}{\eta_{g}^{2}}\E\left[\left\|\nabla_{\bx} \Phi(\bx, \blambda)\right\|^{2}\right] + \frac{12\tau^{2}}{\eta_{g}^{2}}\left(1+\chi\right)\zeta^{2} + \frac{3\tau^{2}}{\eta_g^{2} J}\zeta^{2},
\end{aligned}
\end{equation*}
which completes the proof.
\end{proof}

The next lemma is useful in effectively controlling the drift term in our later analysis.

\begin{lemma}\label{Lemma:x-update-lowerbound-drift}
Suppose $\tau_r = J\,\eta_{\ell}\,\eta_{g}$, and $\eta_{g}\geq 1$, then we have
\begin{equation}
\frac{1}{\tau_{r}}\E\left[\|\bx^{r+1}-\bx^{r}\|^{2}\right] \geq -{\tau_r L_{\bx\bx}^{2}} {\mathcal{E}_r} + \frac{\tau_r}{2}\left\|\nabla_{\bx}\Phi(\bx^{r}, \blambda^{r+1})\right\|^{2},
\end{equation}
where $\nabla_{\bx}\Phi(\bx^{r}, \blambda^{r+1})$ is defined as
\begin{equation}
    \nabla_{\bx}\Phi(\bx^{r}, \blambda^{r+1}) = \sum_{i=1}^{N}\lambda_i^{r+1}\nabla f_i(\bx^{r}).
\end{equation}
\end{lemma}


\begin{proof}
In start with, we analyze $\frac{1}{4\tau_{r}}\|\bx^{r+1}-\bx^{r}\|^{2} $   based on the local updates, i.e.,
\begin{equation*}
\begin{aligned}
&\quad\,\,\frac{1}{\tau_{r}}\E\left[\|\bx^{r+1}-\bx^{r}\|^{2}\right]\\
&= {\tau_r}\E\left[\Big\|\frac{1}{J}\sum_{i=1}^{N}\sum_{j=1}^{J}\lambda_i^{r+1}g_i(\bu^{r}_{i, j-1})\Big\|^{2}\right] \\
& \geq {\tau_r}\E\left[\Big\|\frac{1}{J}\sum_{i=1}^{N}\sum_{j=1}^{J}\lambda_i^{r+1}\nabla f_i(\bu^{r}_{i, j-1})\Big\|^{2}\right]  \\
&\geq -{\tau_r}\E\left[\Big\|\frac{1}{J}\sum_{i=1}^{N}\sum_{j=1}^{J}\lambda_i^{r+1}\nabla f_i(\bu^{r}_{i, j-1}) - \sum_{i=1}^{N}\lambda_i^{r+1}\nabla f_i(\bx^{r})\Big\|^{2}\right] + \frac{\tau_r}{2}\E\left[\left\|\nabla_{\bx}\Phi(\bx^{r}, \blambda^{r+1})\right\|^{2}\right] \\
&\geq -{\tau_r}\frac{1}{J}\sum_{i=1}^{N}\sum_{j=1}^{J}\lambda_i^{r+1}\E\left[\left\|\nabla f_i(\bu^{r}_{i, j-1}) - \nabla f_i(\bx^{r})\right\|^{2}\right] + \frac{\tau_r}{2}\E\left[\left\|\nabla_{\bx}\Phi(\bx^{r}, \blambda^{r+1})\right\|^{2}\right] \\
&\geq -{\tau_r L_{\bx\bx}^{2}}\underbrace{\frac{1}{J}\sum_{i=1}^{N}\sum_{j=1}^{J}\lambda_i^{r+1}\E\left[\left\|\bu^{r}_{i, j-1} - \bx^{r} \right\|^{2}\right]}_{\mathcal{E}_r} + \frac{\tau_r}{2}\E\left[\left\|\nabla_{\bx}\Phi(\bx^{r}, \blambda^{r+1})\right\|^{2}\right]\\
&= -{\tau_r L_{\bx\bx}^{2}} {\mathcal{E}_r} + \frac{\tau_r}{2}\E\left[\left\|\nabla_{\bx}\Phi(\bx^{r}, \blambda^{r+1})\right\|^{2}\right],
\end{aligned}
\end{equation*}
which completes the proof.
\end{proof}

The next two lemmas focus on the primal update and dual update, respectively.
\begin{lemma}\label{Lemma:lamba-update-optimal-confidtion}
Suppose $\tau_r = J\,\eta_{\ell}\,\eta_{g}$, and $\eta_{g}\geq 1$, then we have
\begin{equation}\label{eq:useful-lemma-apd-lambda-update}
\begin{aligned}
&\psi(\blambda^{r+1}) - \langle{\bs}^{r}, \blambda^{r+1}\rangle \\
\leq &\,\psi(\blambda) - \langle{\bs}^{r}, \blambda\rangle + \frac{1}{\sigma_r}\left[\mathrm{D}(\blambda, \blambda^{r})-\mathrm{D}(\blambda, \blambda^{r+1})-\mathrm{D}(\blambda^{r+1}, \blambda^{r})\right] - \frac{\mu_{\blambda}}{2}\|\blambda_{r+1} - \blambda\|^{2}.
\end{aligned}
\end{equation}
\end{lemma}
\begin{proof}
Based on Property 1 in \citet{tseng2008accelerated}, and $\mathrm{D}(\blambda, \blambda^{\prime})= \|\blambda - \blambda^{\prime}\|^{2}/2$.
\end{proof}




\begin{lemma}\label{Lemma:x-update-optimal-confidtion}
Suppose $\tau_r = J\,\eta_{\ell}\,\eta_{g}$, and $\eta_{g}\geq 1$, then we have
\begin{equation}\label{eq:useful-lemma-apd-x-update}
    \E\left[\Big\langle \Delta\bx^{r}, \bx^{r+1} - \bx\Big\rangle\right] \leq  \frac{1}{\tau_r}\E\left[\mathrm{D}(\bx, \bx^{r})-\mathrm{D}(\bx, \bx^{r+1})-\mathrm{D}(\bx^{r+1}, \bx^{r})\right],
\end{equation}
and 
\begin{equation}
\begin{aligned}
&\E\left[\Big\langle \Delta{\bx}^{r}, \bx^{r+1} - \bx\Big\rangle\right]\\
=\,& \underbrace{\E\left[\Big\langle \Delta{\bx}^{r}, \bx^{r} - \bx\Big\rangle\right]}_{\cT_1} +  
\underbrace{\E\left[\Big\langle \widetilde{\Delta}{\bx}^{r}, \bx^{r+1} - \bx^{r}\Big\rangle\right]}_{\cT_2} + \underbrace{\E\left[\Big\langle \Delta{\bx}^{r} - \widetilde{\Delta}{\bx}^{r}, \bx^{r+1} - \bx^{r}\Big\rangle\right]}_{\cT_3},
\end{aligned}
\end{equation}
where
\begin{equation}
\begin{aligned}
    \cT_1 \geq \,& \E\left[{\Phi(\bx^{r}, \blambda^{r+1})} - {\Phi(\bx, \blambda^{r+1})}\right] + \frac{\mu_{\bx}}{4}\E\left[\|\bx^{r}-\bx\|^{2}\right] - L_{\bx\bx}{\mathcal{E}_{r}},\\
    \cT_2 \geq \,& \E\left[{\Phi(\bx^{r+1}, \blambda^{r+1})} - {\Phi(\bx^{r}, \blambda^{r+1})}\right]  - 2L_{\bx\bx}\E\left[\|\bx^{r+1}-\bx^{r}\|^{2}\right] - 2L_{\bx\bx}\mathcal{E}_{r},\\
    \cT_3 \geq \, &-\frac{2\chi\,\tau_r}{J}\zeta^{2} - \frac{1}{4\tau_r}\E\left[\mathrm{D}(  \bx^{r+1}, \bx^{r})\right],
\end{aligned}
\end{equation}
and ${\Delta}{\bx}^{r}$ and $\widetilde{\Delta}{\bx}^{r}$ are defined as
\begin{equation}\label{eq:appendix-delta-x-r-def}
    {\Delta}{\bx}^{r} = \frac{1}{J}\sum_{i=1}^{N}\sum_{j=1}^{J}\lambda_i^{r+1} g_i(\bu^{r}_{i, j-1}), \,\,\,
    \widetilde{\Delta}{\bx}^{r} = \E\left[\Delta\bx^{r}\right] = \frac{1}{J}\sum_{i=1}^{N}\sum_{j=1}^{J}\lambda_i^{r+1}\E\left[\nabla f_i(\bu^{r}_{i, j-1})\right].
\end{equation}
\end{lemma}




\begin{proof}
Based on Property 1 in \citet{tseng2008accelerated}, for the update step of $\bx^{r+1}$, we have
\begin{equation}
    \E\left[\Big\langle \sum_{i=1}^{N}\lambda_i^{r+1}\Delta\bu^{r}_{i}, \bx^{r+1} - \bx\Big\rangle\right] \leq  \frac{1}{\tau_r}\E\left[\mathrm{D}(\bx, \bx^{r})-\mathrm{D}(\bx, \bx^{r+1})-\mathrm{D}(\bx^{r+1}, \bx^{r})\right],
\end{equation}
then we analyze the term $\Delta{\bx}^{r} = \sum_{i=1}^{N}\lambda_i^{r+1}\Delta\bu^{r}_{i}$, i.e.,
\begin{equation}
\begin{aligned}
\sum_{i=1}^{N}\lambda_i^{r+1}\Delta\bu^{r}_{i}
&= \frac{1}{J}\sum_{i=1}^{N}\sum_{j=1}^{J}\lambda_i^{r+1}\left(g_i(\bu^{r}_{i, j-1}) - \hat{\bc}_i^{r} + \hat{\bc}^{r}\right) \\
&= \frac{1}{J}\sum_{i=1}^{N}\sum_{j=1}^{J}\lambda_i^{r+1}g_i(\bu^{r}_{i, j-1})  -  \frac{1}{J}\sum_{i=1}^{N}\sum_{j=1}^{J}\lambda_i^{r+1}\hat{\bc}_i^{r} +  \frac{1}{J}\sum_{i=1}^{N}\sum_{j=1}^{J}\lambda_i^{r+1} \hat{\bc}^{r} \\
&= \frac{1}{J}\sum_{i=1}^{N}\sum_{j=1}^{J}\lambda_i^{r+1}g_i(\bu^{r}_{i, j-1}).
\end{aligned}
\end{equation}
Next we decompose $\E\left[\Big\langle \Delta{\bx}^{r}, \bx^{r+1} - \bx\Big\rangle\right]$ as follows,
\begin{equation}
\begin{aligned}
&\E\left[\Big\langle \Delta{\bx}^{r}, \bx^{r+1} - \bx\Big\rangle\right]\\
=\,& \underbrace{\E\left[\Big\langle \Delta{\bx}^{r}, \bx^{r} - \bx\Big\rangle\right]}_{\cT_1} +  
\underbrace{\E\left[\Big\langle \widetilde{\Delta}{\bx}^{r}, \bx^{r+1} - \bx^{r}\Big\rangle\right]}_{\cT_2} + \underbrace{\E\left[\Big\langle \Delta{\bx}^{r} - \widetilde{\Delta}{\bx}^{r}, \bx^{r+1} - \bx^{r}\Big\rangle\right]}_{\cT_3}.
\end{aligned}
\end{equation}
We then analyze the upper bound for $|\cT_3|$, i.e.,
\begin{equation}
\begin{aligned}
|\cT_3| &= \E\left[\big|\langle \Delta{\bx}^{r} - \widetilde{\Delta}{\bx}^{r}, \bx^{r+1} - \bx^{r}\rangle\big|\right] \\
&\leq {\tau_r} \E\left[\| \Delta{\bx}^{r} - \widetilde{\Delta}{\bx}^{r}\|^{2}\right] + \frac{1}{4\tau_r}\E\left[\|  \bx^{r+1} - \bx^{r}\|^{2}\right]\\
&\leq \frac{2\chi\,\tau_r}{J} \zeta^{2} + \frac{1}{4\tau_r}\E\left[\|  \bx^{r+1} - \bx^{r}\|^{2}\right].
\end{aligned}
\end{equation}
Next, we analyze term $\cT_1$, i.e.,
\begin{equation*}
\begin{aligned}
\cT_1=\,&\E\left[\Big\langle \Delta{\bx}^{r}, \bx^{r} - \bx\Big\rangle\right] = \E\left[\Big\langle \widetilde{\Delta}{\bx}^{r}, \bx^{r} - \bx\Big\rangle\right] \\
=\,& \E\Big[\Big\langle \frac{1}{J}\sum_{i=1}^{N}\sum_{j=1}^{J}\lambda_i^{r+1}\nabla f_i(\bu^{r}_{i, j-1}), \bx^{r} - \bx\Big\rangle\Big]\\
\geq& \frac{1}{J}\sum_{i, j} \lambda_i^{r+1}\E\left[f_i(\bx^{r}) - f_i(\bx)+\frac{\mu_{\bx}}{4}\|\bx^{r}-\bx\|^{2}-L_{\bx\bx}\|\bu_{i,j-1}^{r} -\bx^{r}\|^{2}\right] \\
=& \E\left[\sum_{i} \lambda_i^{r+1}f_i(\bx^{r}) - \sum_{i} \lambda_i^{r+1}f_i(\bx) + \frac{\mu_{\bx}}{4}\|\bx^{r}-\bx\|^{2} - L_{\bx\bx}\frac{1}{J}\sum_{i,j} \lambda_i^{r+1}\|\bu_{i,j-1}^{r} -\bx^{r}\|^{2}\right]  \\
=& \E\left[{\Phi(\bx^{r}, \blambda^{r+1})} - {\Phi(\bx, \blambda^{r+1})}\right] + \frac{\mu_{\bx}}{4}\E\left[\|\bx^{r}-\bx\|^{2}\right] - L_{\bx\bx}{\mathcal{E}_{r}},
\end{aligned}
\end{equation*}
where we apply the perturbed strong convexity lemma (Lemma~\ref{lemma:perturb-strong-convexity}) for the first inequality. 

We then analyze term $\cT_2$, 
\begin{equation*}
\begin{aligned}
\cT_2 =\,& \E\left[\Big\langle \widetilde{\Delta}{\bx}^{r}, \bx^{r+1} - \bx^{r}\Big\rangle\right] \\
=\,& \E\Big[\Big\langle \frac{1}{J}\sum_{i=1}^{N}\sum_{j=1}^{J}\lambda_i^{r+1}\nabla f_i(\bu^{r}_{i, j-1}), \bx^{r+1} - \bx^{r}\Big\rangle\Big]\\
\geq\,& \E\left[{\Phi(\bx^{r+1}, \blambda^{r+1})} - {\Phi(\bx^{r}, \blambda^{r+1})} + \frac{\mu_{\bx}}{4}\|\bx^{r+1}-\bx^{r}\|^{2} - {\frac{L_{\bx\bx}}{J}\sum_{i,j} \lambda_i^{r+1}\|\bu_{i,j-1}^{r} -\bx^{r+1}\|^{2}}\right]\\
\geq\,& \E\left[{\Phi(\bx^{r+1}, \blambda^{r+1})} - {\Phi(\bx^{r}, \blambda^{r+1})} + \left(\frac{\mu_{\bx}}{4} - 2L_{\bx\bx}\right)\|\bx^{r+1}-\bx^{r}\|^{2}\right]   - 2L_{\bx\bx}\mathcal{E}_r \\
\geq\,& \E\left[{\Phi(\bx^{r+1}, \blambda^{r+1})} - {\Phi(\bx^{r}, \blambda^{r+1})}\right]  - 2L_{\bx\bx}\E\left[\|\bx^{r+1}-\bx^{r}\|^{2}\right] - 2L_{\bx\bx}\mathcal{E}_{r},
\end{aligned}
\end{equation*}
where we apply the perturbed strong convexity lemma (Lemma~\ref{lemma:perturb-strong-convexity}) for the first inequality and apply $\|\bx + \by\|^{2}\leq 2\|\bx\|^{2} + 2\|\by\|^{2}$ for the second inequality.  This completes our proof.
\end{proof}
