\begin{center}
    {\Large\bf Appendix} 
\end{center}

\section{Proof for Lemma 1}
\mylemma*

\begin{proof}
First, consider the scenario where channel pairs exhibit consistent importance ranking, specifically, either $x_i>x_j \wedge y_i>y_j$ or $x_i<x_j \wedge y_i<y_j$. In the case where $x_i > x_j \wedge y_i > y_j$, we obtain:
\begin{align}
\lim_{\alpha  \to +\infty } \frac{e^{\alpha(x_i-x_j)}-e^{-\alpha(x_i-x_j)}}{e^{\alpha(x_i-x_j)}+e^{-\alpha(x_i-x_j)}} = 1,
\quad
\lim_{\alpha  \to +\infty } \frac{e^{\alpha(y_i-y_j)}-e^{-\alpha(y_i-y_j)}}{e^{\alpha(y_i-y_j)}+e^{-\alpha(y_i-y_j)}} = 1. 
\nonumber 
\end{align}
On the other hand, if $x_i < x_j \wedge y_i < y_j$, we have:
\begin{align}
\lim_{\alpha  \to +\infty } \frac{e^{\alpha(x_i-x_j)}-e^{-\alpha(x_i-x_j)}}{e^{\alpha(x_i-x_j)}+e^{-\alpha(x_i-x_j)}} = -1,
\quad
\lim_{\alpha  \to +\infty } \frac{e^{\alpha(y_i-y_j)}-e^{-\alpha(y_i-y_j)}}{e^{\alpha(y_i-y_j)}+e^{-\alpha(y_i-y_j)}} = -1.
\nonumber 
\end{align}
Hence, when $x_i > x_j \wedge y_i > y_j$ or $x_i < x_j \wedge y_i < y_j$, the following conclusion holds:
\begin{align}
\lim_{\alpha  \to +\infty } \frac{e^{\alpha(x_i-x_j)}-e^{-\alpha(x_i-x_j)}}{e^{\alpha(x_i-x_j)}+e^{-\alpha(x_i-x_j)}}\frac{e^{\alpha(y_i-y_j)}-e^{-\alpha(y_i-y_j)}}{e^{\alpha(y_i-y_j)}+e^{-\alpha(y_i-y_j)}} = 1.
\label{proof_con}
\end{align}
Second, consider the scenario where channel pairs exhibit inconsistent importance ranking, that is, either $x_i>x_j \wedge y_i<y_j$ or $x_i<x_j \wedge y_i>y_j$. In the case where $x_i>x_j \wedge y_i<y_j$, we obtain:
\begin{align}
\lim_{\alpha  \to +\infty } \frac{e^{\alpha(x_i-x_j)}-e^{-\alpha(x_i-x_j)}}{e^{\alpha(x_i-x_j)}+e^{-\alpha(x_i-x_j)}} = 1,
\quad
\lim_{\alpha  \to +\infty } \frac{e^{\alpha(y_i-y_j)}-e^{-\alpha(y_i-y_j)}}{e^{\alpha(y_i-y_j)}+e^{-\alpha(y_i-y_j)}} = -1.
\nonumber 
\end{align}
On the other hand, if $x_i<x_j \wedge y_i>y_j$, we have:
\begin{align}
\lim_{\alpha  \to +\infty } \frac{e^{\alpha(x_i-x_j)}-e^{-\alpha(x_i-x_j)}}{e^{\alpha(x_i-x_j)}+e^{-\alpha(x_i-x_j)}} = -1,
\quad
\lim_{\alpha  \to +\infty } \frac{e^{\alpha(y_i-y_j)}-e^{-\alpha(y_i-y_j)}}{e^{\alpha(y_i-y_j)}+e^{-\alpha(y_i-y_j)}} = 1.
\nonumber 
\end{align}
Hence, when $x_i > x_j \wedge y_i < y_j$ or $x_i < x_j \wedge y_i > y_j$, the following conclusion holds:
\begin{align}
\lim_{\alpha  \to +\infty } \frac{e^{\alpha(x_i-x_j)}-e^{-\alpha(x_i-x_j)}}{e^{\alpha(x_i-x_j)}+e^{-\alpha(x_i-x_j)}}\frac{e^{\alpha(y_i-y_j)}-e^{-\alpha(y_i-y_j)}}{e^{\alpha(y_i-y_j)}+e^{-\alpha(y_i-y_j)}} = -1.
\label{proof_discon}
\end{align}
When considering all channel pairs, combining Eq. \eqref{proof_con} and Eq. \eqref{proof_discon}, it is evident that:
\begin{align}
\lim_{\alpha  \to +\infty }\Tilde{\tau}_\alpha(\bx,\by) &=\lim_{\alpha  \to +\infty }\frac{1}{N_0} \sum_{i=2}^{n}\sum_{j=1}^{i-1}\frac{e^{\alpha(x_i-x_j)}-e^{-\alpha(x_i-x_j)}}{e^{\alpha(x_i-x_j)}+e^{-\alpha(x_i-x_j)}} \frac{e^{\alpha(y_i-y_j)}-e^{-\alpha(y_i-y_j)}}{e^{\alpha(y_i-y_j)}+e^{-\alpha(y_i-y_j)}}\nonumber \\
&=\frac{N_{\text{con}}-N_{\text{dis}}}{N_0}\nonumber \\
&=\tau (\bx, \by),
\nonumber 
\end{align}
where $N_{\text{con}}$ represents the total count of channel pairs with consistent importance ranking, $N_{\text{dis}}$ represents the count of channel pairs with inconsistent importance ranking.
\end{proof}









    
