\subsection{Proof of Theorem~\ref{thm:convergence}}\label{app:PPM-EM}
We start by introducing some notation. Let $L^{(t)} \in \mathcal{L}$ denote the linear subspace that contains the iterate $\bm{v}_{t}$ in Algorithm~\ref{alg:PPM}. 
Define the linear subspace $F^{(t)} = \mathsf{conv}(L^{(t)} \cup L^{(t+1)} \cup L_{*})$ as the convex hull of $L^{(t)},L^{(t+1)}$ and $L_{*}$. Let
\[
    \widehat{\bm{v}}_{F^{(t)}} = \argmax_{\bm{v} \in F^{(t)} \cap \mathcal{S}^{d-1}} \bm{v}^{\top} \widehat{\bm{\Sigma}} \bm{v}.
\] 
Now we state three lemmas and defer their proofs to subsections~\ref{proof-lemma-prop:F-est},~\ref{proof-lemma-equivalence-of-v} and~\ref{proof-lemma-dist-vF-v'}. 

\begin{lemma} \label{prop:F-est}
Under the setting of linear structure condition~\ref{cond:linear-structure}, for any linear subspace $F$ such that $\bm{v}_* \in L_* \subseteq F$, let 
\[
    \widehat{\bm{v}}_F = \argmax_{\bm{v} \in F \cap \mathcal{S}^{d-1}} \bm{v}^{\top} \bm{\widehat{\Sigma}} \bm{v}^{\top}.
\]
If the eigen-gap $\lambda$ satisfies $\lambda > 2 \rho(\bm{W}, F)$, then 
\begin{align*}
    \|\widehat{\bm{v}}_F - \bm{v}_*\|_2 \leq \frac{\rho(\bm{W}, F)}{\lambda - 2\rho(\bm{W}, F) }.
\end{align*}
\end{lemma}

\begin{lemma}\label{equivalence-of-v}
Let $\{\bm{v}_{t+1}\}_{t=0}^{T}$ be iterates in Algoritm~\ref{alg:PPM}. Then for each $0\leq t \leq T$, we have that
\[
    \bm{v}_{t+1} = \argmin_{\bm{v} \in \mathcal{M} \cap \mathcal{S}^{d-1}} \bigg\| \bm{v} - \frac{\widehat{\bm{\Sigma}}_{F^{(t)}} \bm{v}_{t} }{\| \widehat{\bm{\Sigma}}_{F^{(t)}} \bm{v}_{t} \|_{2}} \bigg\|_{2}, 
\]
i.e., replacing $\widehat{\bm{\Sigma}} \bm{v}_{t}$ by $\widehat{\bm{\Sigma}}_{F^{(t)}} \bm{v}_{t}$ equivalently without changing the left-hand-side result $\bm{v}_{t+1} $. 
\end{lemma}
\begin{lemma}\label{distance-vF-v'}
Let $\lambda_{1}^{F^{(t)}},\lambda_{2}^{F^{(t)}}$ be the first and the second eigenvalues of $\widehat{\bm{\Sigma}}_{F^{(t)}}$. Let 
\begin{align*}
 & ~ \widehat{\kappa}_{F^{(t)}} = \lambda_{2}^{F^{(t)}}/\lambda_{1}^{F^{(t)}},\quad \alpha_{t} = \langle \widehat{\bm{v}}_{F^{(t)}} , \bm{v}_{*} \rangle, \quad \bm{v}_{t+1}' = \frac{\widehat{\bm{\Sigma}}_{F^{(t)}} \bm{v}_{t} }{\| \widehat{\bm{\Sigma}}_{F^{(t)}} \bm{v}_{t} \|_{2}}.
\end{align*}
Then we have 
\[
    \left\| \widehat{\bm{v}}_{F^{(t)}} - \bm{v}_{t+1}' \right\|_{2} \leq \frac{\widehat{\kappa}_{F^{(t)}}}{\alpha_{t}} \cdot \left\| \bm{v}_{t} - \bm{v}_{*} \right\|_{2} + 
    \frac{\widehat{\kappa}_{F^{(t)}}}{\alpha_{t}} \cdot \frac{\rho(\bm{W}, F^{(t)})}{ \lambda - 2\rho(\bm{W}, F^{(t)})}.
\]
\end{lemma}
We are now ready to prove Theorem~\ref{thm:convergence} using Lemma~\ref{prop:F-est}, Lemma~\ref{equivalence-of-v} and Lemma~\ref{distance-vF-v'}.
\begin{proof}
We claim that if $\bm{v}_{t} \in \mathbb{G}(\lambda)$ then

\begin{align}\label{claim-proof-convergence}
	\| \bm{v}_{t+1} - \bm{v}_{*} \|_{2} \leq \frac{1}{2} \cdot \| \bm{v}_{t} - \bm{v}_{*} \|_{2} + \frac{2.5\rho(\bm{W},F^{*})}{\lambda - 2\rho(\bm{W},F^{*})}.
\end{align}
We defer the proof of inequality~\eqref{claim-proof-convergence} to the end. Now we prove Theorem~\ref{thm:convergence} by induction and using inequality~\eqref{claim-proof-convergence}.\\
\textbf{Base case:} $t=0$. Since $\bm{v}_{0} \in \mathbb{G}(\lambda)$ by assumption, then inequality~\eqref{ineq-thm-convergence} follows immediately from inequality~\eqref{claim-proof-convergence}. \\
\textbf{Induction:} Suppose inequality~\eqref{ineq-thm-convergence} holds for $0 \leq t \leq k$. To reduce the notational burden, we use the shorhand
\[
    \epsilon_{*} = \frac{2.5\rho(\bm{W},F^{*})}{\lambda - 2\rho(\bm{W},F^{*})}.
\]
Then by applying inequality~\eqref{ineq-thm-convergence} recursively, we obtain that
\begin{align}\label{recursive-ineq}
    \|\bm{v}_{k+1} - \bm{v}_{*} \|_{2} \leq \frac{1}{2^{k+1}} \cdot \| \bm{v}_{0} - \bm{v}_{*} \|_{2} +  \sum_{t=0}^{k}\frac{1}{2^{t}}\cdot \epsilon_{*}.
\end{align}
We then consider two cases.\\
\textbf{Case 1:} $\| \bm{v}_{0} - \bm{v}_{*} \|_{2} \leq 2\epsilon_{*}$. Then we obtain that 
\[
\|\bm{v}_{k+1} - \bm{v}_{*} \|_{2} \leq \big( \sum_{t=0}^{k}\frac{1}{2^{t}} + \frac{1}{2^{k}} \big) \epsilon_{*} \leq 2\epsilon_{*}.
\]
Using the fact that $\bm{v}_{k+1},\bm{v}_{*}$ are unit norm vectors, we obtain that 
\[
    \langle\bm{v}_{k+1}, \bm{v}_{*} \rangle \geq  1 - 2\epsilon_{*}^{2} \geq 1-2\epsilon_{*} \geq 1 - \frac{5\rho(\bm{W},F^{*})}{\lambda - 2\rho(\bm{W},F^{*})},
\]
where in the last inequality we use $\epsilon_{*}<1$ by the inequality~\eqref{eigen-gap-condition}. Consequently, by the assumption that $\lambda$ is large enough so that inequality~\eqref{eigen-gap-condition} holds, we obtain that $\bm{v}_{k+1} \in \mathbb{G}(\lambda)$. Then the induction step follows immediately from claim~\eqref{claim-proof-convergence}.\\
\textbf{Case 2:} $\| \bm{v}_{0} - \bm{v}_{*} \|_{2} > 2\epsilon_{*}$. In this case, we obtain that
\[
     \sum_{t=0}^{k}\frac{1}{2^{t}} \cdot \epsilon_{*} \leq 2\cdot(1-2^{-(k+1)}) \cdot \epsilon_{*} \leq (1-2^{-(k+1)}) \cdot \| \bm{v}_{0} - \bm{v}_{*} \|_{2}.
\]
Combining with inequality~\eqref{recursive-ineq}, we obtain that
\begin{align*}
    \|\bm{v}_{k+1} - \bm{v}_{*} \|_{2} 
    \leq & ~ \|\bm{v}_{0} - \bm{v}_{*} \|_{2} + \sum_{t=0}^{k}\frac{1}{2^{t}} \cdot \epsilon_{*} - (1-2^{-(k+1)}) \cdot \| \bm{v}_{0} - \bm{v}_{*} \|_{2} \\
    \leq & ~ \|\bm{v}_{0} - \bm{v}_{*} \|_{2}.
\end{align*}
Consequently, we obtain $\langle\bm{v}_{k+1}, \bm{v}_{*} \rangle \geq \langle\bm{v}_{0}, \bm{v}_{*} \rangle$. Then $\bm{v}_{k+1} \in \mathbb{G}(\lambda)$. Then the induction step follows immediately from inequality~\eqref{claim-proof-convergence}.
We now apply Lemmas~\ref{prop:F-est},~\ref{equivalence-of-v} and~\ref{distance-vF-v'} to prove the claim~\eqref{claim-proof-convergence}.
\paragraph{Proof of inequality~\eqref{claim-proof-convergence}}
Let $\widehat{\kappa}_{F^{(t)}},\alpha_{t}$ and $\bm{v}_{t+1}'$ be defined as in Lemma~\ref{distance-vF-v'}. Using the triangular inequality, we obtain that
\begin{align*}
\|\bm{v}_{t+1} - \bm{v}_{*} \|_{2} 
\leq & ~ \|\bm{v}_{t+1} - \bm{v}_{t+1}' \|_{2}  + \|\bm{v}_{t+1}' - \bm{v}_{*} \|_{2} \\ 
\overset{(1)}{\leq} & ~ 2\|\bm{v}_{t+1}' - \bm{v}_{*} \|_{2} \leq 2\|\bm{v}_{t+1}' - \widehat{\bm{v}}_{F^{(t)}} \|_{2} + 2\|\widehat{\bm{v}}_{F^{(t)}} - \bm{v}_{*} \|_{2},
\end{align*}
where in step $(1)$ we use $\|\bm{v}_{t+1} - \bm{v}_{t+1}' \|_{2} \leq \|\bm{v}_{t+1}' - \bm{v}_{*} \|_{2}$ following directly from Lemma~\ref{equivalence-of-v}. Since $L_{*} \subset F^{(t)}$, using Lemma~\ref{prop:F-est}, we obtain that
\begin{align}\label{part1-proof-claim-thm-convergence}
\|\widehat{\bm{v}}_{F^{(t)}} - \bm{v}_{*} \|_{2} \leq \frac{\rho(\bm{W},F^{(t)})}{\lambda - 2\rho(\bm{W},F^{(t)})} \leq \frac{\rho(\bm{W},F^{*})}{\lambda - 2\rho(\bm{W},F^{*})}.
\end{align}
Combining inequality~\eqref{part1-proof-claim-thm-convergence} with Lemma~\ref{distance-vF-v'}, we obtain that
\begin{align}\label{ineq-one-step-away}
    \|\bm{v}_{t+1} - \bm{v}_{*} \|_{2} \leq & ~ \frac{2\widehat{\kappa}_{F^{(t)}}}{\alpha_{t}} \cdot \left\| \bm{v}_{t} - \bm{v}_{*} \right\|_{2} + 
    \big(\frac{2\widehat{\kappa}_{F^{(t)}}}{\alpha_{t}} + 2\big) \cdot \frac{\rho(\bm{W}, F^{(t)})}{ \lambda - 2\rho(\bm{W}, F^{(t)})}. 
\end{align}
Note that
\begin{align*}
\lambda_{1}^{F^{(t)}} \geq & ~ \bm{v}_{*}^{\top} \widehat{\bm{\Sigma}}_{F^{(t)}} \bm{v}_{*} \\
= & ~ \bm{v}_{*}^{\top} \bm{\Sigma} \bm{v}_{*} + \bm{v}_{*}^{\top} \bm{W} \bm{v}_{*} \geq \lambda + 1 - \rho(\bm{W},F^{(t)}) \quad \text{and}\\
\lambda_{2}^{F^{(t)}} \leq & ~ \lambda_{2}(\bm{\Sigma}_{F^{(t)}}) + \rho(\bm{W},F^{(t)}) \leq \lambda_{2}(\bm{\Sigma}) + \rho(\bm{W},F^{(t)}) \\
= & ~ 1 + \rho(\bm{W},F^{(t)}).
\end{align*}
Moreover, we note that
\begin{align*}
\alpha_{t} = \langle \widehat{\bm{v}}_{F^{(t)}} , \bm{v}_{*} \rangle &= \langle \bm{v}_{t}, \bm{v}_{*} \rangle + \langle \widehat{\bm{v}}_{F^{(t)}} - \bm{v}_{t}, \bm{v}_{*} \rangle \\
&\geq \langle \bm{v}_{t}, \bm{v}_{*} \rangle - \| \widehat{\bm{v}}_{F^{(t)}} - \bm{v}_{t} \|_{2} \\
&\geq \frac{4(1+\rho(\bm{W},F^{*}))}{\lambda+1 - \rho(\bm{W},F^{*})},
\end{align*}
where the last step follows from $\bm{v}_{t} \in \mathbb{G}(\lambda)$ and inequality~\eqref{part1-proof-claim-thm-convergence}.
Putting the pieces together yields
\begin{align}\label{coeff-upper-bound}
    \frac{\widehat{\kappa}_{F^{(t)}}}{\alpha_{t}} = \frac{\lambda_{2}^{F^{(t)}}}{\lambda_{1}^{F^{(t)}} \alpha_{t}} \leq \frac{1}{4}.
\end{align}
Substituting inequality~\eqref{coeff-upper-bound} into inequality~\eqref{ineq-one-step-away} yields the desired result and concludes the proof.
\end{proof}





\subsubsection{Proof of Lemma~\ref{prop:F-est}}\label{proof-lemma-prop:F-est}
\begin{proof}
Note that we have the decomposition
\begin{align*}
	& ~ \widehat{\bm{v}}_F = \alpha \bm{v}_* + \beta \bm{v}_{\bot} \quad \text{such that} \quad \alpha^2 + \beta^2 = 1, \|\bm{v}_*\|_2^2 = \|\bm{v}_{\bot}\|_2^2 = 1, \langle \bm{v}_*, \bm{v}_{\bot}\rangle = 0.
\end{align*}
 By definition, $\widehat{\bm{v}}_F$ is the eigenvector with respect to the largest eigenvalue $\lambda_{\max}(\widehat{\bm{\Sigma}}_F)$ of $\widehat{\bm{\Sigma}}_F$. We obtain that
\begin{align*}
    \bm{v}_{\bot}^{\top} \widehat{\bm{\Sigma}}_F \widehat{\bm{v}}_F &= \lambda_{\max}(\widehat{\bm{\Sigma}}_F) \bm{v}_{\bot}^{\top} \widehat{\bm{v}}_F = \lambda_{\max}(\widehat{\bm{\Sigma}}_F) \cdot \beta \quad \text{and} \\
    \bm{v}_{\bot}^{\top} \widehat{\bm{\Sigma}}_F \widehat{\bm{v}}_F &= \bm{v}_{\bot}^{\top} \widehat{\bm{\Sigma}}_F (\alpha \bm{v}_* + \beta \bm{v}_{\bot}) = \alpha \cdot \bm{v}_{\bot}^{\top} \widehat{\bm{\Sigma}}_F \bm{v}_* + \beta \cdot \bm{v}_{\bot}^{\top} \widehat{\bm{\Sigma}}_F \bm{v}_{\bot}.
\end{align*} 
Consequently, we obtain that
\begin{align}\label{ineq-beta-lemma-F-est}
     |\beta| = & ~ |\alpha| \frac{|\bm{v}_{\bot}^{\top} \widehat{\bm{\Sigma}}_F \bm{v}_*|}{\lambda_{\max}(\widehat{\bm{\Sigma}}_F) - \bm{v}_{\bot}^{\top} \widehat{\bm{\Sigma}}_F \bm{v}_{\bot}} \\
     \overset{(1)}{=} & ~ |\alpha| \frac{| \bm{v}_{\bot}^{\top} \bm{W}_F \bm{v}_*|}{\lambda_{\max}(\widehat{\bm{\Sigma}}_F) - \bm{v}_{\bot}^{\top} \widehat{\bm{\Sigma}}_F \bm{v}_{\bot}} \notag \\
     \leq & ~ |\alpha| \frac{\rho(\bm{W}, F)}{\lambda - 2\rho(\bm{W}, F) }, \notag
\end{align}
where in step $(1)$ we use 
\begin{align*}
	\bm{v}_{\bot}^{\top} \widehat{\bm{\Sigma}}_F \bm{v}_* = & ~ \bm{v}_{\bot}^{\top} \bm{\Sigma}_F \bm{v}_* + \bm{v}_{\bot}^{\top} \bm{W}_F \bm{v}_* \\
	= & ~ (\lambda + 1) \bm{v}_{\bot}^{\top}\bm{v}_* + \bm{v}_{\bot}^{\top} \bm{W}_F \bm{v}_* \\
	= & ~ \bm{v}_{\bot}^{\top} \bm{W}_F \bm{v}_*, 
\end{align*}
and in the last step we use
\begin{align*}
    & ~ \lambda_{\max}(\widehat{\bm{\Sigma}}_F) - \bm{v}_{\bot}^{\top} \widehat{\bm{\Sigma}}_F \bm{v}_{\bot} \\
    \geq & ~ \lambda_{\max}(\widehat{\bm{\Sigma}}_F) - \lambda_2 (\widehat{\bm{\Sigma}}_F) \notag\\
    = & ~ \lambda_{\max}(\bm{\Sigma}_F + \bm{W}_F) - \lambda_2(\bm{\Sigma}_F + \bm{W}_F) \notag\\
    \geq & ~ \lambda_{\max}(\bm{\Sigma}_F) - \lambda_{\max}(\bm{W}_F) - \lambda_2(\bm{\Sigma}_F) - \lambda_{\max}(\bm{W}_F) \notag\\
    = & ~ \lambda_{\max}(\bm{\Sigma}_F) - \lambda_2(\bm{\Sigma}_F) - 2 \rho(\bm{W}, F) \notag\\
    \geq & ~ \lambda - 2 \rho(\bm{W}, F).
\end{align*}
Applying inequality~\eqref{ineq-beta-lemma-F-est} yields
\begin{align*}
    \alpha^2 \left( 1 + \frac{\rho^2(\bm{W}, F)}{(\lambda - 2\rho(\bm{W}, F))^2} \right) \geq \alpha^2 + \beta^2 = 1.
\end{align*}
Consequently we obtain that
\[
    \alpha \geq \frac{1}{\sqrt{ 1 + \frac{\rho^2(\bm{W}, F)}{(\lambda - 2\rho(\bm{W}, F))^2} }} \geq 1 - \frac{\rho^2(\bm{W}, F)}{2(\lambda - 2\rho(\bm{W}, F))^2},
\]
where in the last step we use $1/\sqrt{1+x} \geq 1-x/2$ for $x>0$. Continuing, we obtain that
\begin{align*}
   & ~ \|\widehat{\bm{v}}_F - \bm{v}_*\|_2^2 = 2 - 2 \alpha \leq \frac{\rho^2(\bm{W}, F)}{(\lambda - 2\rho(\bm{W}, F))^2} \\
   \quad \Rightarrow & ~ \|\widehat{\bm{v}}_F - \bm{v}_*\|_2 \leq \frac{\rho(\bm{W}, F)}{\lambda - 2\rho(\bm{W}, F) },
\end{align*}
which completes the proof. 
\end{proof}



\subsubsection{Proof of Lemma~\ref{equivalence-of-v}}\label{proof-lemma-equivalence-of-v}
\begin{proof}
Note that
\begin{align}\label{piece1-proof-lemma-equi}
 \bm{\theta} = \argmin_{\bm{v} \in \mathcal{M} \cap \mathcal{S}^{d-1}} \bigg\| \bm{v} - \frac{\widehat{\bm{\Sigma}}_{F^{(t)}} \bm{v}_{t} }{\| \widehat{\bm{\Sigma}}_{F^{(t)}} \bm{v}_{t} \|_{2}} \bigg\|_{2} = \argmax_{\bm{v} \in \mathcal{M} \cap \mathcal{S}^{d-1}} \langle \bm{v}, \widehat{\bm{\Sigma}}_{F^{(t)}} \bm{v}_{t} \rangle.
\end{align}
Let $L' \in \mathcal{L}$ be the linear subspace such that $\bm{\theta} \in L'$. By definition~\ref{cond:linear-structure}, there are $\mathcal{B}_{L'},\mathcal{B}_{F^{(t)}} \subseteq \mathcal{B} = \{\phi_1,\cdots,\phi_{d}\}$ such that $L' = \mathsf{span}(\mathcal{B}_{L'})$ and $F^{(t)} = \mathsf{span}(\mathcal{B}_{F^{(t)}})$. Hence we obtain that $\bm{P}_{L'} \bm{P}_{F^{(t)}} = \bm{P}_{L' \cap F^{(t)}}$, where $L' \cap F^{(t)} = \mathsf{span}(\mathcal{B}_{L'} \cap \mathcal{B}_{F^{(t)}})$. Consequently, we obtain that
we obtain that
\[
    \bm{\theta} = \frac{\bm{P}_{L'} \widehat{\bm{\Sigma}}_{F^{(t)}} \bm{v}_{t} }{ \| \bm{P}_{L'} \widehat{\bm{\Sigma}}_{F^{(t)}} \bm{v}_{t} \|_{2}} = \frac{\bm{P}_{L'} \bm{P}_{F^{(t)}} \widehat{\bm{\Sigma}} \bm{v}_{t} }{ \| \bm{P}_{L'} \widehat{\bm{\Sigma}}_{F^{(t)}} \bm{v}_{t} \|_{2}} = \frac{\bm{P}_{L' \cap F^{(t)}}  \widehat{\bm{\Sigma}} \bm{v}_{t} }{ \| \bm{P}_{L'} \widehat{\bm{\Sigma}}_{F^{(t)}} \bm{v}_{t} \|_{2}}.
\] 
It immediately shows that $\bm{\theta} \in F^{(t)}$. On the other hand, it follows from Algorithm~\ref{alg:PPM} that 
\begin{align*}
    \bm{v}_{t+1}^{\mathcal{M}} &= \argmin_{\bm{v} \in \mathcal{M}} \bigg\|\bm{v} - \frac{\widehat{\bm{\Sigma}} \bm{v}_{t}}{\|\widehat{\bm{\Sigma}} \bm{v}_{t}\|_{2}}\bigg\|_{2}^{2} \\
    &= \argmin_{\bm{v} \in \mathcal{M}} \|\bm{v}\|_{2}^{2} - 2\langle \bm{v}/\|\bm{v}\|_{2}, \widehat{\bm{\Sigma}} \bm{v}_{t} \rangle \cdot \frac{\|\bm{v}\|_{2}}{\|\widehat{\bm{\Sigma}} \bm{v}_{t}\|_{2}}  + 1.
\end{align*}
Note that the minimization over $\|\bm{v}\|_{2}$ and $\bm{v}/\|\bm{v}\|_{2}$ are independent. Consequently, we obtain that
\begin{align}\label{piece2-proof-lemma-equi}
     \bm{v}_{t+1} = \frac{\bm{v}_{t+1}^{\mathcal{M}}}{\|\bm{v}_{t+1}^{\mathcal{M}}\|_{2}} = \argmax_{\bm{v} \in \mathcal{M} \cap \mathcal{S}^{d-1}} \langle \bm{v}, \widehat{\bm{\Sigma}} \bm{v}_{t} \rangle.
\end{align}
Putting the pieces together yields that
\begin{align*}
    \langle \bm{\theta}, \widehat{\bm{\Sigma}}_{F^{(t)}} \bm{v}_{t} \rangle \overset{(1)}{=} & ~ \langle \bm{\theta}, \widehat{\bm{\Sigma}} \bm{v}_{t} \rangle \overset{(2)}{\leq} \langle \bm{v}_{t+1}, \widehat{\bm{\Sigma}} \bm{v}_{t} \rangle \\
    \overset{(3)}{=} & ~ \langle \bm{v}_{t+1}, \widehat{\bm{\Sigma}}_{F^{(t)}} \bm{v}_{t} \rangle \overset{(4)}{\leq} \langle \bm{\theta}, \widehat{\bm{\Sigma}}_{F^{(t)}} \bm{v}_{t} \rangle,
\end{align*}
where step $(1)$ and $(3)$ follow from $\bm{\theta},\bm{v}_{t+1} \in F^{(t)}$, step $(2)$ follows from inequality~\eqref{piece2-proof-lemma-equi} and step $(4)$ follows from inequality~\eqref{piece1-proof-lemma-equi}. Consequently, we obtain that
\[
    \langle \bm{v}_{t+1}, \widehat{\bm{\Sigma}}_{F^{(t)}} \bm{v}_{t} \rangle = \langle \bm{\theta}, \widehat{\bm{\Sigma}}_{F^{(t)}} \bm{v}_{t} \rangle.
\]
Since the optimal solution in the last step of inequality~\eqref{piece1-proof-lemma-equi} is unique, we conclude that $\bm{v}_{t+1} = \bm{\theta}$.
\end{proof}







\subsubsection{Proof of Lemma~\ref{distance-vF-v'}}\label{proof-lemma-dist-vF-v'}
\begin{proof}
By definition, we obtain that
\begin{align*}
    \left\| \widehat{\bm{v}}_{F^{(t)}} - \bm{v}_{t + 1}' \right\|_2^2 = & ~ 2 - 2 \langle \widehat{\bm{v}}_{F^{(t)}}, \bm{v}_{t + 1}' \rangle \\
    = & ~ 2 - 2 \left\langle \widehat{\bm{v}}_{F^{(t)}},  \frac{\widehat{\bm{\Sigma}}_{F^{(t)}} \bm{v}_t}{\|\widehat{\bm{\Sigma}}_{F^{(t)}} \bm{v}_t\|_2} \right\rangle. 
\end{align*} 
Note that we have the decomposition
\begin{align*}
	& ~ \bm{v}_{t} = \alpha_{t} \cdot \widehat{\bm{v}}_{F^{(t)}} + \beta_{t} \cdot \widehat{\bm{v}}_{\perp}, \\
    \text{where} & ~ \langle \widehat{\bm{v}}_{\perp}, \widehat{\bm{v}}_{F^{(t)}} \rangle = 0,\quad \|\widehat{\bm{v}}_{\perp}\|_{2} = 1\quad \text{and} \quad \beta_{t} = \langle \bm{v}_{t}, \widehat{\bm{v}}_{\perp} \rangle. 
\end{align*}
Using the decomposition in the display above, we have 
\begin{align*}
    \left\langle \widehat{\bm{v}}_{F^{(t)}},  \frac{\widehat{\bm{\Sigma}}_{F^{(t)}} \bm{v}_t}{\|\widehat{\bm{\Sigma}}_{F^{(t)}} \bm{v}_t\|_2} \right\rangle = & ~ \frac{\widehat{\bm{v}}_{F^{(t)}}^{\top} \widehat{\bm{\Sigma}}_{F^{(t)}} (\alpha_t \widehat{\bm{v}}_{F^{(t)}} + \beta_t \widehat{\bm{v}}_{\perp}) }{\|\widehat{\bm{\Sigma}}_{F^{(t)}} (\alpha_t \widehat{\bm{v}}_{F^{(t)}} + \beta_t \widehat{\bm{v}}_{\perp}) \|_2} \\
    = & ~ \frac{\alpha_t \lambda_{1}^{F^{(t)}}}{\sqrt{ \alpha_t^2 (\lambda_{1}^{F^{(t)}})^2 + \beta_t^2 \|\widehat{\bm{\Sigma}}_{F^{(t)}} \bm{v}_{\perp}\|_2^2 }},
\end{align*}
where in the last step we use $\langle \widehat{\bm{v}}_{F^{(t)}}, \widehat{\bm{\Sigma}}_{F^{(t)}} \widehat{\bm{v}}_{\perp} \rangle = 0$. Continuing, we obtain that
\begin{align*}
    \frac{\alpha_t \lambda_{1}^{F^{(t)}}}{ \sqrt{ \alpha_t^2 (\lambda_{1}^{F^{(t)}})^2 + \beta_t^2 \|\widehat{\bm{\Sigma}}_{F^{(t)}} \bm{v}_{\perp}\|_2^2 } }  
    \geq & ~ \frac{\alpha_t \lambda_{1}^{F^{(t)}}}{ \sqrt{ \alpha_t^2 (\lambda_{1}^{F^{(t)}})^2 + \beta_t^2 (\lambda_{2}^{F^{(t)}})^2 } }  \\
    = & ~ \frac{1}{ \sqrt{ 1 + \frac{\beta_t^2}{\alpha_t^2} \widehat{\kappa}_{F^{(t)}}^2 } } \\
    \geq & ~ 1 - \frac{\beta_t^2}{\alpha_t^2} \frac{\widehat{\kappa}_{F^{(t)}}^2}{2},
\end{align*}
where we use $\|\widehat{\bm{\Sigma}}_{F^{(t)}} \bm{v}_{\perp}\|_2 \leq \lambda_{2}^{F^{(t)}}$ in the first step and we use $\frac{1}{\sqrt{1 + x}} \geq 1 - \frac{x}{2}$ for any $x \geq 0$ in the last step. Putting the three pieces together yields
\begin{align*}
    \left\| \widehat{\bm{v}}_{F^{(t)}} - \bm{v}_{t + 1}' \right\|_2^2 \leq & ~ \frac{\beta_t^2 \widehat{\kappa}_{F^{(t)}}^2 }{\alpha_t^2} = \frac{\widehat{\kappa}_{F^{(t)}}^2 (1 + \alpha_t)}{2 \alpha_t^2} \left\| \widehat{\bm{v}}_{F^{(t)}} - \bm{v}_{t} \right\|_2^2 \\
    \leq & ~ \frac{\widehat{\kappa}_{F^{(t)}}^2}{\alpha_t^2} \left\| \widehat{\bm{v}}_{F^{(t)}} - \bm{v}_{t} \right\|_2^2,
\end{align*}
where the final inequality holds since $1 + \alpha_t \leq 2$. Hence we get 
\begin{align*}
    \left\| \widehat{\bm{v}}_{F^{(t)}} - \bm{v}_{t + 1}' \right\|_2 \leq & ~ \frac{\widehat{\kappa}_{F^{(t)}}}{\alpha_t} \left\| \widehat{\bm{v}}_{F^{(t)}} - \bm{v}_{t} \right\|_2 \\
    \leq & ~ \frac{\widehat{\kappa}_{F^{(t)}}}{\alpha_t} \left\| \widehat{\bm{v}}_{F^{(t)}} - \bm{v}_* \right\|_2  + \frac{\widehat{\kappa}_{F^{(t)}}}{\alpha_t} \left\| \bm{v}_* - \bm{v}_{t} \right\|_2 \\
    \leq & ~ \frac{\widehat{\kappa}_{F^{(t)}}}{\alpha_t} \frac{\rho(\bm{W}, F^{(t)})}{\lambda - 2\rho(\bm{W}, F^{(t)})} + \frac{\widehat{\kappa}_{F^{(t)}}}{\alpha_t} \left\| \bm{v}_* - \bm{v}_{t} \right\|_2, 
\end{align*}
where the final inequality follows from Lemma~\ref{prop:F-est}. 
\end{proof}




















