
  The first property -- the positivity of the probability mass function of
  $\widetilde{\nu}^{j}$ -- is immediate from its definition.

  To simplify the notation, denote in what follows
  \begin{equation}
    K^{j}(x,y) = \exp\left(
    \frac{\phi_{\psi^{j}}(x) + \psi^{j}(y) - c(x,y)}{\lambda}\right).
  \end{equation}
  With this notation, recall that
  $$
    \widehat{\nu}^{j}_{\vecpsi}(y^{j}_{l})
    = \frac{1}{n}\sum_{i=1}^{n}\nu^{j}(y^{j}_{l})K(X_{i},y^{j}_{l}).
  $$
  The above is a sum of $n$ non-negative random variables bounded by one
  with expectation
  $$
    (\nu' )^{j}(y^{j}_{l})
    = \mathbf{E}_{X \sim \mu_{\vecpsi}'}\left[
      \nu^{j}(y^{j}_{l})
    \right]
  $$
  It follows by Hoeffding's inequality
  and the union bound that with probability
  at least $1-\delta$ the following holds for any
  $j \in \{1,\dots,k\}$ and any $l \in \{1, \dots, m_{j}\}$:
  \begin{equation}
    \label{eq:hoeffding}
    \left|
      \widehat{\nu}_{\vecpsi}(y^{j}_{l})
      - (\nu' )^{j}(y^{j}_{l})
    \right|
    \leq \sqrt{\frac{2\log\left(\frac{2m}{\delta}\right)}{n}}.
  \end{equation}
  In particular, the above implies that
  \begin{align}
    \|\widetilde{\nu}^{j}_{\vecpsi} - \nu^{j}_{\vecpsi}\|_{\mathrm{TV}}
    &\leq 2\zeta +
    (1-\zeta)
    \|\widetilde{\nu}^{j}_{\vecpsi} - \nu^{j}_{\vecpsi}\|_{\mathrm{TV}}
    \\
    &\leq 2\zeta +
    (1-\zeta)
    \|\widetilde{\nu}^{j}_{\vecpsi} - (\nu')^{j}\|_{\mathrm{TV}}
    + (1-\zeta)\|(\nu')^{j} - \nu^{j}_{\vecpsi}\|_{\mathrm{TV}}
    \\
    &\leq 2\zeta +
    \|\widetilde{\nu}^{j}_{\vecpsi} - (\nu')^{j}\|_{\mathrm{TV}}
    + \|(\nu')^{j} - \nu^{j}_{\vecpsi}\|_{\mathrm{TV}}
    \\
    &\leq 2\zeta + m_{j}\varepsilon_{\mu}
    + m_{j}
    \sqrt{\frac{2\log\left(\frac{2m}{\delta}\right)}{n}}.
  \end{align}
  Notice that the above bound can be made arbitrarily close to
  $m_{j}\varepsilon_{\mu}$ by taking a large enough $n$ and a small enough
  $\zeta$.
  This proves the second property of
  Definition~\ref{dfn:approximate-sinkhorn-oracle}.

  To prove the third property,
  observe that
  \begin{align}
    \mathbf{E}_{Y \sim \nu^{j}}\left[
      \frac{\nu^{j}_{\vecpsi}(Y)}{\widetilde{\nu}^{j}_{\vecpsi}(Y)}
    \right]
    &=
    \mathbf{E}_{Y \sim \nu^{j}}\left[
      \frac{\widehat{\nu}^{j}_{\vecpsi}(Y)}
      {\widetilde{\nu}^{j}_{\vecpsi}(Y)}
      + \frac{\nu^{j}_{\vecpsi}(Y) - \widehat{\nu}^{j}_{\vecpsi}(Y)
      }{\widetilde{\nu}^{j}_{\vecpsi}(Y)}
    \right]
    \\
    &\leq
    \mathbf{E}_{Y \sim \nu^{j}}\left[
      \frac{1}{1-\zeta} + \frac{\nu^{j}_{\vecpsi}(Y) - \widehat{\nu}^{j}_{\vecpsi}(Y)
      }{\widetilde{\nu}^{j}_{\vecpsi}(Y)}
    \right]
    \\
    &\leq
    \mathbf{E}_{Y \sim \nu^{j}}\left[
      1
      + \frac{\zeta}{1-\zeta}
      + \frac{\left|\nu^{j}_{\vecpsi}(Y) -
        \widehat{\nu}^{j}_{\vecpsi}(Y)\right|
      }{\widetilde{\nu}^{j}_{\vecpsi}(Y)}
    \right]
    \\
    &\leq
    1 +
    \frac{\zeta}{1-\zeta}
    + \frac{1}{\zeta}
    \|\nu^{j}_{\vecpsi}(Y) -
    \widehat{\nu}^{j}_{\vecpsi}(Y)\|_{\mathrm{TV}}
    \\
    &\leq
    1
    +
    2\zeta
    + \frac{1}{\zeta}
    \left(m_{j}\varepsilon_{\mu} + m_{j}
      \sqrt{\frac{2\log\left(\frac{2m}{\delta}\right)}{n}}
    \right).
  \end{align}
  This concludes the proof of the third property.

  It remains to prove the fourth property of
  Definition~\ref{dfn:approximate-sinkhorn-oracle}.
  Observe that for any $y,y'$ we have
  \begin{align}
    &\left(
      \psi^{j}(y) - \eta\lambda\log\frac{\widetilde{\nu}^{j}(y)}{\nu^{j}(y)}
    \right)
    -
    \left(
      \psi^{j}(y') - \eta\lambda\log\frac{\widetilde{\nu}^{j}(y')}{\nu^{j}(y')}
    \right)
    \\
    &=
    \left(\psi^{j}(y) - \psi^{j}(y')\right)
    + \eta\lambda\log
    \left(
    \frac
    {
      \zeta + (1-\zeta)\frac{1}{n}\sum_{i=1}^{n}K^{j}(X_{i}, y')
    }
    {
      \zeta + (1-\zeta)\frac{1}{n}\sum_{i=1}^{n}K^{j}(X_{i}, y)
    }
    \right)
    \\
    &=
    \left(\psi^{j}(y) - \psi^{j}(y')\right)
    + \eta\lambda\log
    \left(
    \frac
    {
      \frac{\zeta}{1-\zeta} + \frac{1}{n}\sum_{i=1}^{n}K^{j}(X_{i}, y')
    }
    {
      \frac{\zeta}{1-\zeta} + \frac{1}{n}\sum_{i=1}^{n}K^{j}(X_{i}, y)
    }
    \right)
    \\
    &\leq
    \left(\psi^{j}(y) - \psi^{j}(y')\right)
    + \eta\lambda\log
    \left(
    \frac
    {
      \frac{\zeta}{1-\zeta} + \exp\left(\frac{c_{\infty}(\mathcal{X}) +
        \psi^{j}(y') - \psi^{j}(y)}{\lambda}
      \right)\frac{1}{n}\sum_{i=1}^{n}K^{j}(X_{i}, y)
    }
    {
      \frac{\zeta}{1-\zeta} + \frac{1}{n}\sum_{i=1}^{n}K^{j}(X_{i}, y)
    }
    \right).
    \label{eq:psi-oscilation-zeta-bound-intermediate}
  \end{align}
  Now observe that for any $a,b > 0$ the function $g:[0,\infty) \to (0,\infty)$
  defined by $g(x) = (x+a)/(x+b)$ is increasing if $a < b$ and decreasing if $a
  \geq b$. Thus, $g$ is maximized either at zero or at infinity.
  It thus follows that
  \begin{align}
    &\eta\lambda\log\left(
      \frac
    {
      \frac{\zeta}{1-\zeta}
      +
      \exp\left(\frac{c_{\infty}(\mathcal{X})}{\lambda}
      \right)
      \frac{1}{n}\sum_{i=1}^{n}K^{j}(X_{i}, y)
    }
    {
      \frac{\zeta}{1-\zeta} + \frac{1}{n}\sum_{i=1}^{n}K^{j}(X_{i}, y)
    }
    \right)
    \\
    &\leq
    \begin{cases}
      \eta c_{\infty}(\mathcal{X})
      -\eta(\psi^{j}(y) - \psi^{j}(y'))
      &\text{if }
      \exp\left(\frac{c_{\infty}(\mathcal{X})}{\lambda}
      \right) \geq 1
      \\
      0&\text{otherwise.}
    \end{cases}
  \end{align}
  This proves the claim and completes the proof of this lemma.
  \hfill\qed


