Recall that for any non-negative integer $t$ we have
\begin{equation}
  \mu_{t}(dx) = Z_{t}^{-1}
  \exp\left(-\frac{\sum_{j=1}^{k}
  w_{j}\phi^{j}_{t}(x)}{\tau}\right) \piref(dx).
\end{equation}
where $Z_{t}$ is the normalizing constant defined by
\begin{equation}
  Z_{t} = \int_{\mathcal{X}}
  \exp\left(-\frac{\sum_{j=1}^{k}
  w_{j}\phi^{j}_{t}(x)}{\tau}\right) \piref(dx).
\end{equation}
With the notation introduced above, we have
\begin{equation}
  E(\vecpsi_{t})
  = \sum_{j=1}^{k}w_{j}\mathbf{E}_{Y \sim \nu^{j}}\left[\psi^{j}_{t}(Y)\right]
  - \tau \log Z_{t}.
\end{equation}
Hence,
\begin{align}
  E(\vecpsi_{t+1}) - E(\vecpsi_{t})
  &=
  \sum_{j=1}^{k}
  w_{j}\mathbf{E}_{Y \sim \nu^{j}}\left[\psi^{j}_{t+1}(Y) - \psi^{j}_{t}(Y)\right]
  - \tau \log \frac{Z_{t+1}}{Z_{t}}.
  \\
  &=
  \eta\lambda\sum_{j=1}^{k}
  w_{j}\mathbf{E}_{Y \sim \nu^{j}}\left[\log\frac{d\nu^{j}}{d\nu^{j}_{t}}(Y)\right]
  - \tau \log \frac{Z_{t+1}}{Z_{t}}.
  \\
  &=
  \min\left(\lambda, \tau\right)
  \sum_{j=1}^{k}
  w_{j}
  \kl{\nu^{j}}{\nu^{j}_{t}}
  - \tau \log \frac{Z_{t+1}}{Z_{t}}.
\end{align}
Therefore, to prove Proposition~\ref{prop:one-step-improvement} it suffices to
show that the inequality
\begin{equation}
  \label{eq:prop-one-step-improvement-sufficient}
  \log \frac{Z_{t+1}}{Z_{t}} \leq 0
\end{equation}
holds for any $t \geq 0$.
We will complete the proof of Proposition~\ref{prop:one-step-improvement}
using the following lemma, the proof of which is
deferred to the end of this section.

\begin{lemma}
  \label{lemma:log-Z-ratio-bound}
  Let $(\vecpsi_{t})_{t \geq 0}$ be any sequence of the form
  $$
    \psi_{t+1}^{j} = \psi_{t}^{j} + \eta\lambda\log(\Delta^{j}_{t}),
  $$
  where for $j \in \{1,\dots,k\}$,  $(\Delta_{t}^{j})_{t \geq 0}$ is an
  arbitrary sequence of strictly positive functions
  and $\eta = \min(1, \tau/\lambda)$.
  Then, for any $t \geq 0$ it holds that
  \begin{equation}
    \tau\log\frac{Z_{\vecpsi_{t+1}}}{Z_{\vecpsi_{t}}}
    \leq
    \min(\lambda, \tau)
    \log
    \sum_{j=1}^{k}w_{j}
    \mathbf{E}_{Y \sim \nu^{j}_{\vecpsi_{t}}}\left[
      \Delta^{j}_{t}(Y)
    \right].
  \end{equation}
\end{lemma}

To complete the proof of Proposition~\ref{prop:one-step-improvement},
we will apply the above lemma with $\Delta_{t}^{j} = \log
\frac{d\nu^{j}}{d\nu_{t}^{j}}$. Indeed, we have
\begin{align}
  \tau \log \frac{Z_{t+1}}{Z_{t}}
  &\leq
  \min(\lambda,\tau)
  \log
  \sum_{j=1}^{k}w_{j}
  \mathbf{E}_{Y \sim \nu^{j}_{t}}\left[
    \frac{d\nu^{j}}{d\nu_{t}^{j}}(Y)
  \right]
  \\
  &=
  \min(\lambda,\tau)
  \log
  \sum_{j=1}^{k}w_{j}
  \mathbf{E}_{Y \sim \nu^{j}}\left[
    1
  \right]
  \\
  &=
  0.
\end{align}
By \eqref{eq:prop-one-step-improvement-sufficient}, the proof of
Proposition~\ref{prop:one-step-improvement} is complete.
\hfill\qed

%%%%%%%%%%%%%%%%%%%%%%%%%%%%%%%%%%%%%%%%%%%%%%%%%%%%%%%%%%%%%%%%%%%%%%%%%%%%%%%
\subsection{Proof of Lemma~\ref{lemma:log-Z-ratio-bound}}

We will break down the proof
with the help of the following lemma, the proof of which can be found in
Section~\ref{sec:proof-of-Zt-ratio-lemma}.

\begin{lemma}
  \label{lemma:zt-ratio}
  For any sequence $(\vecpsi_{t})_{t \geq 0}$ and any $t \geq 0$
  it holds that
  \begin{equation}
    \log
    \frac{Z_{\vecpsi_{t+1}}}{Z_{\vecpsi{t}}}
    \leq
    \begin{cases}
      \frac{\lambda}{\tau}
      \log
      \sum_{j=1}^{k}
      w_{j}
      \mathbf{E}_{X \sim \mu_{t}}\left[
          \exp\left(\frac{-\phi^{j}_{t+1}(X)+\phi^{j}_{t}(X)}{\tau}
          \right)^{\tau/\lambda}
        \right]
        & \text{ if }\tau \geq \lambda,\\
      \log
      \sum_{j=1}^{k}
      w_{j}
      \mathbf{E}_{X \sim \mu_{t}}\left[
          \exp\left(\frac{-\phi^{j}_{t+1}(X)+\phi^{j}_{t}(X)}{\tau}
          \right)
        \right]
        & \text{ if }\tau < \lambda,
    \end{cases}
  \end{equation}
  where $\vecphi_{t} = \vecphi_{\vecpsi_{t}}$
  and $\mu_{t}(dx) =
  Z_{\vecpsi_{t}}^{-1}
  \exp(-\sum_{j=1}^{k}w_{j}\phi_{t}^{j}(x)/\tau)\piref(dx)$.
\end{lemma}

Observe that the sequence $(\vecpsi_{t})_{t\geq0}$ of the form stated in
Lemma~\ref{lemma:log-Z-ratio-bound} satisfies, for any
for any $j \in \{1,\dots,k\}$ and any $t \geq 0$,
\begin{equation}
    \exp\left(
      \frac{-\phi^{j}_{t+1}+\phi^{j}_{t}}{\tau}
    \right)
    =
    \exp\left(
      -\frac{\lambda}{\tau}
      \log\frac{d\mu_{t}}{d\tilde{\mu}^{j}_{t}}
    \right)
    =
    \left(\frac{d\tilde{\mu}^{j}_{t}}{d\mu_{t}}\right)^{\lambda/\tau},
\end{equation}
where
\begin{align}
  \frac{d\tilde{\mu}^{j}_{t}}{d\mu_{t}}(x)
  &=
  \int_{\mathcal{X}}
  \nu(dy)\exp\left(\frac{\psi^{j}_{t+1}(y) + \phi^{j}_{t}(x) - c(x,y)}{\lambda}\right)
  \\
  &=
  \int_{\mathcal{X}}
  \nu^{j}(dy) \Delta_{t}^{j}(y)^{\eta}\exp\left(
    \frac{\psi^{j}_{t}(y) + \phi^{j}_{t}(x) - c(x,y)}{\lambda}\right).
\end{align}
Hence, by Lemma~\ref{lemma:zt-ratio}
we have
\begin{align}
  &\log\frac{Z_{\vecpsi_{t+1}}}{Z_{\vecpsi_{t}}}
  \\
  &\leq
  \frac{1}{\tau}\min(\lambda, \tau)
  \sum_{j=1}^{k}
  w_{j}
  \mathbf{E}_{X \sim \mu_{t}}\Bigg[
  \\&\quad\quad
    \left(
    \int_{\mathcal{X}}
    \nu^{j}(dy)\Delta_{t}^{j}(y)^{\eta}\exp\left(
      \frac{\psi^{j}_{t}(y) + \phi^{j}_{t}(X) - c(X,y)}{\lambda}\right)
    \right)^{\max(1, \lambda/\tau)}
  \Bigg].
  \label{eq:Zt-ratio-bound-before-case-splitting}
\end{align}
We split the remaining proof into two cases:
$\tau \geq \lambda$ and $\tau < \lambda$.

\paragraph{The case \texorpdfstring{$\tau \geq \lambda$}{tau >= lambda}.}
When $\tau \geq \lambda$, we have $\max(1,\lambda/\tau) = 1$ and $\eta =
\min(1,\tau/\lambda) = 1$. Thus,  \eqref{eq:Zt-ratio-bound-before-case-splitting}
yields
\begin{align}
  &\log\frac{Z_{\vecpsi_{t+1}}}{Z_{\vecpsi_{t}}}
  \\
  &\leq
  \frac{1}{\tau}\min(\lambda, \tau)
  \log
  \sum_{j=1}^{k}
  w_{j}
  \mathbf{E}_{X \sim \mu_{t}}\left[
    \int_{\mathcal{X}}
    \nu^{j}(dy)\Delta_{t}^{j}(y)\exp\left(
      \frac{\psi^{j}_{t}(y) + \phi^{j}_{t}(X) - c(X,y)}{\lambda}\right)
  \right]
  \\
  &=
  \frac{1}{\tau}\min(\lambda, \tau)
  \log
  \sum_{j=1}^{k}
  w_{j}
  \left[
    \int_{\mathcal{X}}
    \mu_{t}(dx)
    \int_{\mathcal{X}}
    \nu^{j}(dy)\Delta_{t}^{j}(y)\exp\left(
      \frac{\psi^{j}_{t}(y) + \phi^{j}_{t}(X) - c(X,y)}{\lambda}\right)
  \right]
  \\
  &=
  \frac{1}{\tau}\min(\lambda, \tau)
  \log
  \sum_{j=1}^{k}
  w_{j}
  \left[
    \int_{\mathcal{X}}
    \Delta_{t}^{j}(y)\nu^{j}(dy)
    \int_{\mathcal{X}}
    \exp\left(
      \frac{\psi^{j}_{t}(y) + \phi^{j}_{t}(X) - c(X,y)}{\lambda}\right)
    \mu_{t}(dx)
  \right]
  \\
  &=
  \frac{1}{\tau}\min(\lambda, \tau)
  \log
  \sum_{j=1}^{k}
  w_{j}
  \left[
    \int_{\mathcal{X}}
    \Delta_{t}^{j}(y)\nu^{j}(dy)
    \frac{d\nu^{j}_{\vecpsi_{t}}}{d\nu^{j}}(y)
  \right]
  \\
  &=
  \frac{1}{\tau}\min(\lambda, \tau)
  \log
  \sum_{j=1}^{k}
  w_{j}
  \mathbf{E}_{Y \sim \nu^{j}_{\vecpsi_{t}}}
  \left[
    \Delta^{j}_{t}(y)
  \right].
\end{align}
This completes the proof of Lemma~\ref{lemma:log-Z-ratio-bound}
when $\tau \geq \lambda$.

\paragraph{The case \texorpdfstring{$\tau < \lambda$}{tau < lambda}.}

For $j \in \{1, \dots, k\}$ and any $x \in \mathcal{X}$ define the measure
$\rho_{x}$ by
\begin{equation}
  \rho^{j}_{x}(dy) =
  \nu^{j}(dy)
  \exp\left(\frac{\psi^{j}_{t}(y) + \phi^{j}_{t}(x) -
  c(x,y)}{\lambda}\right).
\end{equation}
By the definition of $\phi^{j}_{t}$, we have
\begin{align}
  &\int_{\mathcal{X}} \rho^{j}_{x}(dy)
  \\
  &=
  \int_{\mathcal{X}}
    \nu(dy)
    \exp\left(\frac{\psi^{j}_{t}(y) - c(x,y)}{\lambda}\right)
    \exp\left(\frac{\phi^{j}_{t}(x)}{\lambda}\right)
  \\
  &=
  \int_{\mathcal{X}}
    \nu(dy)
    \exp\left(\frac{\psi^{j}_{t}(y) - c(x,y)}{\lambda}\right)
    \exp\left(-\log\int_{\mathcal{X}}
      \nu^{j}(dy')
      \exp\left(\frac{\psi^{j}_{t}(y') - c(x,y')}{\lambda}\right)
    \right)
  \\
  &=
  1
\end{align}
In particular, $\rho_{x}$ is a probability measure.
Hence,
\eqref{eq:Zt-ratio-bound-before-case-splitting} can be rewritten as
\begin{align}
  \log \frac{Z_{\vecpsi_{t+1}}}{Z_{\vecpsi_{t}}}
  &\leq
  \log
  \sum_{j=1}^{k}
  w_{j}
  \mathbf{E}_{X \sim \mu_{t}}\left[
    \mathbf{E}_{Y \sim \rho^{j}_{X}}\left[
    \Delta^{j}_{t}(Y)^{\eta}
    \bigg\vert X
  \right]^{\lambda/\tau}
\right]
\end{align}
Because $\lambda/\tau > 1$, the function $x \mapsto x^{\lambda/\tau}$ is
convex. Applying Jensen's inequality to the conditional expectation and using
the fact that $\eta\lambda/\tau = 1$, it follows that
\begin{align}
  \log \frac{Z_{\vecpsi_{t+1}}}{Z_{\vecpsi_{t}}}
  &\leq
  \log
  \sum_{j=1}^{k}
  w_{j}
  \mathbf{E}_{X \sim \mu_{t}}\left[
    \mathbf{E}_{Y \sim \rho^{j}_{X}}\left[
    \Delta^{j}_{t}(Y)
    \bigg\vert X
  \right]
  \right]
  \\
  &=
  \log
  \sum_{j=1}^{k}
  w_{j}
  \int_{\mathcal{X}}
    \mu_{t}(dx)
  \int_{\mathcal{X}}
  \Delta_{t}^{j}(y)
  \exp\left(\frac{\psi^{j}_{t}(y) + \phi^{j}_{t}(x) -
    c(x,y)}{\lambda}\right)
    \nu(dy).
    \label{eq:proof-of-one-step-improvement-proposition-pre-Fubini-step}
\end{align}
By the definition of $\nu^{j}_{\vecpsi_{t}}$ we have
\begin{equation}
  \frac{d\nu^{j}_{\vecpsi_{t}}}{d\nu^{j}}(y)
  =
  \int_{\mathcal{X}}
  \exp\left(\frac{\psi^{j}_{t}(y) + \phi^{j}_{t}(x) -
  c(x,y)}{\lambda}\right)\mu_{t}(dx).
\end{equation}
Interchanging the order of integration in
\eqref{eq:proof-of-one-step-improvement-proposition-pre-Fubini-step}
and plugging in the above equation yields
\begin{align}
  \log \frac{Z_{\vecpsi_{t+1}}}{Z_{\vecpsi_{t}}}
  &\leq
  \log
  \sum_{j=1}^{k}
  w_{j}
  \int_{\mathcal{X}}
  \left[
    \int_{\mathcal{X}}
    \exp\left(\frac{\psi^{j}_{t}(y) + \phi^{j}_{t}(x) -
    c(x,y)}{\lambda}\right)
    \mu_{t}(dx)
  \right]
  \Delta^{j}_{t}(y)
  \nu^{j}(dy)
  \\
  &=
  \log
  \sum_{j=1}^{k}
  w_{j}
  \int_{\mathcal{X}}
  \left[
    \frac{d\nu^{j}_{\vecpsi_{t}}}{d\nu^{j}}(y)
  \right]
  \Delta_{t}^{j}(y)
  \nu^{j}(dy)
  \\
  &=
  \log
  \sum_{j=1}^{k}
  w_{j}
  \mathbf{E}_{Y \sim \nu^{j}_{\vecpsi_{t}}}\left[
    \Delta^{j}_{t}(Y)
  \right].
\end{align}
This completes the proof of Lemma~\ref{lemma:log-Z-ratio-bound}.
\hfill\qed



%%%%%%%%%%%%%%%%%%%%%%%%%%%%%%%%%%%%%%%%%%%%%%%%%%%%%%%%%%%%%%%%%%%%%%%%%%%%%%%
\subsection{Proof of Lemma~\ref{lemma:zt-ratio}}
\label{sec:proof-of-Zt-ratio-lemma}
To simplify the notation, denote $Z_{t} = Z_{\vecpsi_{t}}$.
Let $x \in \mathcal{X}$ and $t \geq 0$. We have $\mu_{t} \ll \mu_{t+1}$ with
the Radon-Nikodym derivative $d\mu_{t+1}/d\mu_{t}$ given by
\begin{align}
  \frac{d\mu_{t+1}}{d\mu_{t}}(x)
  &= \frac{Z_{t}}{Z_{t+1}} \exp\left(
    \frac{-\sum_{j=1}^{k}w_{k}(\phi^{j}_{t+1}(x) - \phi^{j}_{t}(x))}{\tau}
  \right)
  \\
  &=
  \frac{Z_{t}}{Z_{t+1}} \prod_{j=1}^{k}
    \exp\left(
      \frac{-\phi^{j}_{t+1}(x) + \phi^{j}_{t}(x)}{\tau}
    \right)^{w_{j}}.
\end{align}
Multiplying both sides by $Z_{t+1}/Z_{t}$ and taking expectations with respect
to $\mu_{t}$ yields
\begin{align}
  \frac{Z_{t+1}}{Z_{t}}
  &=
  \mathbf{E}_{X \sim \mu_{t+1}}\left[
    \frac{Z_{t+1}}{Z_{t}}
  \right]
  \\
  &=
  \mathbf{E}_{X \sim \mu_{t}}\left[
    \frac{Z_{t+1}}{Z_{t}}
    \frac{d\mu_{t+1}}{d\mu_{t}}(X)
  \right]
  \\
  &=
  \mathbf{E}_{X \sim \mu_{t}}\left[
    \prod_{j=1}^{k}
    \exp\left(
      \frac{-\phi^{j}_{t+1}(X) + \phi^{j}_{t}(X)}{\tau}
    \right)^{w_{j}}
  \right].
\end{align}
In the case $\tau < \lambda$, the proof is complete by the Artihmetic-Geometric
mean inequality (recall that $w_{j} > 0$ for $j=1,\dots,k$ and
$\sum_{j=1}^{k}w_{j} = 1$).
On the other hand, if $\tau \geq \lambda$ then $x \mapsto x^{\lambda/\tau}$ is
concave. Hence, it follows that
\begin{align}
  \log
  \frac{Z_{t+1}}{Z_{t}}
  &=
  \log
  \mathbf{E}_{X \sim \mu_{t}}\left[
    \left(
    \prod_{j=1}^{k}
    \exp\left(
      \frac{-\phi^{j}_{t+1}(X) + \phi^{j}_{t}(X)}{\tau}
    \right)^{w_{j}\tau/\lambda}
    \right)^{\lambda/\tau}
  \right]
  \\
  &\leq
  \log
  \mathbf{E}_{X \sim \mu_{t}}\left[
    \left(
    \prod_{j=1}^{k}
    \exp\left(
      \frac{-\phi^{j}_{t+1}(X) + \phi^{j}_{t}(X)}{\tau}
    \right)^{w_{j}\tau/\lambda}
    \right)
  \right]^{\lambda/\tau}
  \\
  &=
  \frac{\lambda}{\tau}
  \log
  \mathbf{E}_{X \sim \mu_{t}}\left[
    \left(
    \prod_{j=1}^{k}
    \exp\left(
      \frac{-\phi^{j}_{t+1}(X) + \phi^{j}_{t}(X)}{\tau}
    \right)^{w_{j}\tau/\lambda}
    \right)
  \right]
  \\
  &\leq
  \sum_{j=1}^{k}
  w_{j}
  \mathbf{E}_{X \sim \mu_{t}}\left[
    \exp\left(
      \frac{-\phi^{j}_{t+1}(X) + \phi^{j}_{t}(X)}{\tau}
    \right)^{\tau/\lambda}
  \right],
\end{align}
where the final step follows via the Arithmetic-Geometric mean
inequality. This completes the proof of Lemma~\ref{lemma:zt-ratio}.
\hfill\qed
%%%%%%%%%%%%%%%%%%%%%%%%%%%%%%%%%%%%%%%%%%%%%%%%%%%%%%%%%%%%%%%%%%%%%%%%%%%%%%%

