To simplify the notation throughout this proof, for each $j \in \{1,\dots,k\}$
denote $\phi^{j} = \phi_{\psi^{j}}$. We have
\begin{align}
  \label{eq:suboptimality-to-kl-proof-first-equation}
  E^{\vecnu,w}_{\lambda, \tau}(\vecpsi^{*})
  - E^{\vecnu,w}_{\lambda,\tau}(\vecpsi)
  =
  \sum_{j=1}^{k}w_{j}
  \mathbf{E}_{Y \sim \nu^{j}}\left[(\psi^{*})^{j}(Y) -
  \psi^{j}(Y)\right]
  - \tau
  \log
  \frac{Z_{\vecpsi^{*}}}{Z_{\vecpsi}}.
\end{align}
Observe that for any $x \in \mathcal{X}$ it holds that
\begin{align}
  \frac{d\mu_{\vecpsi}}{d\mu_{\vecpsi^{*}}}(x)
  =
  \frac{Z_{\vecpsi^{*}}}{Z_{\vecpsi}}
  \exp\left(
    -\frac{
      \sum_{j=1}^{k}w_{j}(\phi^{j}(x) - (\phi^{*})^{j}(x))
    }{\tau}
  \right).
\end{align}
Hence,
\begin{align}
  \tau\log
  \frac{Z_{\vecpsi^{*}}}{Z_{\vecpsi}}
  &=
  \tau\log\mathbf{E}_{X \sim \mu_{\vecpsi^{*}}}\left[
     \frac{Z_{\vecpsi^{*}}}{Z_{\vecpsi}}
  \right]
  \\
  &=
  \tau\log\mathbf{E}_{X \sim \mu_{\vecpsi^{*}}}\left[
    \frac{d\mu_{\vecpsi}}{d\mu_{\vecpsi^{*}}}(x)
    \exp\left(
      \frac{
        \sum_{j=1}^{k}w_{j}(\phi^{j}(x) - (\phi^{*})^{j}(x))
      }{\tau}
    \right)
  \right]
  \\
  &=
  \tau\log\mathbf{E}_{X \sim \mu_{\vecpsi}}\left[
    \exp\left(
      \frac{
        \sum_{j=1}^{k}w_{j}(\phi^{j}(x) - (\phi^{*})^{j}(x))
      }{\tau}
    \right)
  \right]
  \\
  &=
  \sup_{\mu \ll \mu_{\vecpsi}}\left\{
    \mathbf{E}_{X \sim \mu}\left[
        \sum_{j=1}^{k}w_{j}(\phi^{j}(x) - (\phi^{*})^{j}(x))
    \right]
    - \tau \kl{\mu}{\mu_{\vecpsi}}
  \right\},
  \label{eq:kl-log-mgf-duality}
\end{align}
where in the final expression we have applied the
Donsker-Varadhan variational principle (i.e., convex-conjugate
duality between KL-divergence and cumulant generating functions); therein, the
supremum runs over probability measures $\mu$ absolutely continuous with
respect to $\mu_{\vecpsi}$, and it is attained by $\mu$ defined as
\begin{align}
  \mu(dx)
  &\propto
  \exp\left(
    \frac{1}{\tau}\sum_{j=1}^{k}w_{j}(\phi^{j}(x) - (\phi^{*})^{j}(x))
  \right)\mu_{\vecpsi}(dx)
  \\
  &\propto
  \exp\left(
    \frac{1}{\tau}\sum_{j=1}^{k}w_{j}(\phi^{j}(x) - (\phi^{*})^{j}(x))
  \right)
  \exp\left(
    -\frac{1}{\tau}\sum_{j=1}^{k}w_{j}\phi^{j}(x)
  \right)\piref(dx)
  \\
  &\propto
  \exp\left(
    -\frac{1}{\tau}\sum_{j=1}^{k}w_{j}(\phi^{*})^{j}(x)
  \right)
  \piref(dx)
  = \pi_{\vecpsi^{*}}(dx).
\end{align}
That is, the supremum in \eqref{eq:kl-log-mgf-duality} is attained by $\mu =
\mu_{\vecpsi^{*}}$. Hence, the identity
\eqref{eq:suboptimality-to-kl-proof-first-equation} becomes
\begin{align}
  &E^{\vecnu,w}_{\lambda, \tau}(\vecpsi^{*})
  - E^{\vecnu,w}_{\lambda,\tau}(\vecpsi)
  \\
  &=
  \sum_{j=1}^{k}
  w_{j}
  \mathbf{E}_{Y \sim \nu^{j}}\left[(\psi^{*})^{j}(Y) - \psi^{j}(Y)\right]
  -
  \mathbf{E}_{X \sim \mu_{\vecpsi^{*}}}\bigg[
      \sum_{j=1}^{k}w_{j}(\phi^{j}(X) - (\phi^{*})^{j}(X))
  \bigg]
  \\
  &\quad\quad
  + \tau \kl{\mu_{\vecpsi^{*}}}{\mu_{\vecpsi}}
  \\
  &=
  \sum_{j=1}^{k}
  w_{j}
  \left(
    \mathbf{E}_{Y \sim \nu^{j}}\left[(\psi^{*})^{j}(Y) -
    \psi^{j}(Y)\right]
    +
    \mathbf{E}_{X \sim \mu_{\vecpsi^{*}}}\left[
      (\phi^{*})^{j}(X))
      - \phi^{j}(X)
    \right]
  \right)
  + \tau \kl{\mu_{\vecpsi^{*}}}{\mu_{\vecpsi}}
  \\
  &\geq
  \tau \kl{\mu_{\vecpsi^{*}}}{\mu_{\vecpsi}},
\end{align}
where the final inequality follows by noting that for each $j$ the optimality
of the pair $((\phi^{*})^{j}, (\psi^{*})^{j})$ for the entropic optimal transport
dual objective $E^{\mu_{\vecpsi^{*}}, \nu^{j}}_{\lambda}$ implies
that
\begin{align}
    &\mathbf{E}_{Y \sim \nu^{j}}\left[(\psi^{*})^{j}(Y) -
    \psi^{j}(Y)\right]
    +
    \mathbf{E}_{X \sim \mu_{\vecpsi^{*}}}\left[
      (\phi^{*})^{j}(X)
      - \phi^{j}(X)
    \right]
    \\
    &=
    E^{\mu, \nu^{j}}_{\lambda}((\phi^{*})^{j}, (\psi^{*})^{j})
    - E^{\mu,\nu^{j}}_{\lambda}(\phi^{j}, \psi^{j})
    \geq 0.
\end{align}
The proof of Lemma~\ref{lemma:suboptimality-to-kl} is complete.\hfill\qed

