\section{Proof of the main result}
\label{sec:proofofthemainresult}
Since we deal with both the original and the auxiliary processes in this section, certain notation needs clarifying to avoid possible ambiguity: the process $(\tx_t^\e,\txi_t^\e)$ represents not a generic process with arbitrary bounded $c(x,y)$ but only the auxiliary process with $\tilde c(x,y)$ satisfying \eqref{eq:added term}; 
$\sigma_n$, $\tau_n$ are defined as in \eqref{eq:stopping_times}, and 
$\Tilde\sigma_n$, $\Tilde{\tau}_n$ represent the corresponding stopping time w.r.t. $(\tx_t^\e,\txi_t^\e)$. In \eqref{eq:definition_of_operator_AB}, we defined $\mathcal L_{c}$ on each edge for a generic $c(x,y)$. Here we give a more explicit definition of $\mathcal L_{\tilde c}=\tilde L_k$ on the edge $I_k$:
\begin{align*}
    \tilde L_kf(h)&=\frac{1}{2}A_k(h)f''(h)+\tilde B_k(h)f'(h),\\
    A_k(h)&=\frac{2}{Q_k(h)}\int_{\gamma_k(h)}\frac{1}{|\nabla H(x)|}\int_0^\infty\E_\mu b_h(x,\xi_s)b_h(x,\xi_0)dsdl,\\
    \Tilde B_k(h)&=\frac{1}{Q_k(h)}\int_{\gamma_k(h)}\frac{1}{|\nabla H(x)|}\int_0^\infty\E_\mu\mathrm{div}_x (b_h(x,\xi_s)(b(x,\xi_0)-\nabla^{\perp}H(x)))dsdl.
\end{align*}
One can easily check that this is consistent with the definitions of $\bar A$ and $\bar B_c$ in \eqref{eq:definition_of_operator_AB}, which are the generalizations of the coefficients defined in Section~\ref{sec:mainresult}, and
\begin{equation}
\label{eq6:derivative}
    \frac{1}{2}[A_k(h_k)Q_k(h_k)f'(h_k)]'=\frac{1}{2}A_k(h_k)Q_k(h_k)f''(h_k)+\Tilde B_k(h_k)Q_k(h_k)f'(h_k).
\end{equation}
\begin{lemma}
\label{lem:zeroexpectation}
    For each $f\in \mathcal D$ and all $\e$ sufficiently small, we have $\Expe_{\nu^\e} \int_0^{\sigma_1}\mathcal L_{\Tilde c}f(h(\tx_t^\e))dt=0$.
\end{lemma}
\begin{proof}
    Since the process $(\tx_t^\e,\txi_t^\e)$ on $M\times\mathbb T^m$ is recurrent, and the measure $\lambda\times\mu$ is the invariant measure, by Theorem~2.1 in \cite{Khasminskii}, we have that for any measurable set $A\subset M$,
    \[
        \int_M\chi_A(x)d\lambda(x)=\lambda(A)=(\lambda\times\mu)(A\times\mathbb T^m)=\E_{\nu^\e}\int_0^{\sigma_1}\chi_A(\tx_t^\e)dt.
    \]
    Thus,
    \[
        \int_M \mathcal L_{\Tilde c}f(h(x))d\lambda(x)=\E_{\nu^\e}\int_0^{\sigma_1}\mathcal L_{\Tilde c}f(h(\tx_t^\e))dt.
    \]
    So it suffices to show that the left hand side is zero. By \eqref{eq6:derivative} and \eqref{eq2:gluing_condition},
\begin{align*}
       \int_{M}\mathcal L_{\Tilde c}f(h(x))d\lambda(x)&=\sum_{k=1}^3\int_{I_k} \tilde L_kf(h_k)Q_k(h_k)dh_k\\
       &=\sum_{k=1}^3\int_{I_k}(\frac{1}{2}A_k(h_k)f''(h_k)+\Tilde B_k(h_k)f'(h_k))Q_k(h_k)dh_k\\
       &=\sum_{k=1}^3\int_{I_k}\frac{1}{2}[A_k(h_k)Q_k(h_k)f'(h_k)]'dh_k\\
       &=\frac{1}{2}\sum_{k=1}^3p_k\lim_{h_k\to O}f'(h_k)\\
       &=0.
\end{align*}
%Because $f'$ decays so fast at infinity.
%Where does the inaccessibility play its role? In this statement, seems like we only need A is zero at extremum, but the criterion needs that 1/A is not integrable.
\end{proof}

Let us verify the analogue of \eqref{eq:mg_problem_M} in the case of the auxiliary process $(\tx_t^\e,\txi_t^\e)$.
\begin{proposition}
\label{prop:auxiliary}
For each $f\in \mathcal D$ and $T>0$,
    \begin{equation}
        \E_{(x,y)}[f(h(\tx_{\eta}^\e))-f(h(x))-\int_0^{\eta}\mathcal L_{\Tilde c}f(h(\tx_t^\e))dt]\to0
    \end{equation}
    as $\e\to0$, uniformly in $x\in M$, $y\in\mathbb T^m$, and $\eta$ is a stopping time bounded by $T$.
\end{proposition}
\begin{proof}
We divide the time interval $[0,\eta]$ into visits to the separatrix. Since $\sigma_n\to\infty$,
    \begin{align}
        &|\E_{(x,y)}[f(h(\tx_{\eta}^\e))-f(h(x))-\int_0^{\eta}\mathcal L_{\Tilde c}f(h(\tx_t^\e))dt]|\nonumber\\
        &\leq|\lim_{n\to\infty}\E_{(x,y)}[f(h(\tx_{\tilde\sigma_n}^\e))-f(h(x))-\int_0^{\tilde\sigma_n}\mathcal L_{\Tilde c}f(h(\tx_t^\e))dt]|\nonumber\\
        &\quad+|\lim_{n\to\infty}\E_{(x,y)}\E_{(\tx_{\eta}^\e,\txi_{\eta}^\e)}[f(h(\tx_{\tilde\sigma_n}^\e))-f(h(\tx_0^\e))-\int_0^{\tilde\sigma_n}\mathcal L_{\Tilde c}f(h(\tx_t^\e))dt]|\nonumber\\
        &\leq 2\sup_{(x,y)\in M\times\mathbb T^m}|\E_{(x,y)}[f(H(\tx^\e_{\tilde\sigma}))-f(H(x))-\int_0^{\sigma}{\mathcal L_{\tilde c}} f(H(\tx_s^\e))ds]|\label{eq6:to_separatrx}\\
        &\quad+2\lim_{n\to\infty}\sup_{(x,y)\in\gamma\times\mathbb T^m}|\E_{(x,y)}[f(h(\tx_{\tilde\sigma_n}^\e))-f(h(x))-\int_0^{\sigma_n}\mathcal L_{\tilde c}f(h(\tx_t^\e))dt]|.\label{eq6:between_separatrices}
    \end{align}
    Note that \eqref{eq6:to_separatrx} converges to $0$ due to Proposition~\ref{prop:up_to_separatrix}, and \eqref{eq6:between_separatrices} also converges to $0$ since
    \begin{align*}
        &\lim_{n\to\infty}\sup_{(x,y)\in\gamma\times\mathbb T^m}|\E_{(x,y)}[f(h(\tx_{\tilde\sigma_n}^\e))-f(h(x))-\int_0^{\tilde\sigma_n}\mathcal L_{\tilde c}f(h(\tx_t^\e))dt]|\\
        &\leq\lim_{n\to\infty}\sup_{(x,y)\in\gamma\times\mathbb T^m}\sum_{k=0}^{n-1}|\E_{(x,y)}\int_{\tilde\sigma_k}^{\tilde\sigma_{k+1}}\mathcal L_{\tilde c}f(h(\tx_t^\e))dt|\\
        &\leq\lim_{n\to\infty}\sup_{(x,y)\in\gamma\times\mathbb T^m}\sum_{k=0}^n \left(2\cdot\mathrm{TV}(\nu_{x,y}^{k,\e},\nu^\e)\cdot\sup_{(x',y')\in\gamma\times\mathbb T^m}|\E_{(x',y')}\int_0^{\tilde\sigma_1}\mathcal L_{\tilde c}f(h(\tx_t^\e))dt|\right)\\
        &=0,
    \end{align*}
    where the second inequality is due to Lemma~\ref{lem:zeroexpectation} and the last equality follows from Proposition~\ref{prop:up_to_separatrix}, Lemma~\ref{lem5:expo_ergodicity}, and Proposition~\ref{prop:exit_time_from_separatrix}.
    Thus, the desired result holds.
\end{proof}
\input{proof_from_aux_to_gen.tex}